Move small-step semantics into its own theory
Remove the old messy small-step attempt

vyperSmallStepScript.sml
@@ -1,1976 +1,1046 @@
-open HolKernel boolLib bossLib Parse wordsLib dep_rewrite blastLib
-open listTheory alistTheory finite_mapTheory arithmeticTheory byteTheory
-     pairTheory numposrepTheory stringTheory combinTheory pred_setTheory
-     wordsTheory cv_typeTheory cv_stdTheory cv_transLib
-open vyperAstTheory vfmTypesTheory vfmContextTheory
+open HolKernel boolLib bossLib Parse
+     cv_transLib whileTheory pairTheory combinTheory
+     arithmeticTheory vyperInterpreterTheory
 
 val () = new_theory "vyperSmallStep";
 
-(* TODO: move *)
-Theorem cv_rep_DOMSUB[cv_rep]:
-  from_fmap f (m \\ k) = cv_delete (Num k) (from_fmap f m)
-Proof
-  rw[from_fmap_def, GSYM cv_delete_thm]
-  \\ AP_TERM_TAC
-  \\ DEP_REWRITE_TAC[sptreeTheory.spt_eq_thm]
-  \\ rw[sptreeTheory.wf_fromAList, sptreeTheory.wf_delete]
-  \\ rw[sptreeTheory.lookup_delete, sptreeTheory.lookup_fromAList]
-  \\ rw[DOMSUB_FLOOKUP_THM]
-QED
-
-val () = cv_auto_trans sptreeTheory.size_def;
-
-Theorem cv_ispair_cv_add[simp]:
-  cv_ispair (cv_add x y) = Num 0
-Proof
-  Cases_on`x` \\ Cases_on`y` \\ rw[]
-QED
-
-Theorem c2n_cv_add[simp]:
-  cv$c2n (cv_add v1 v2) = cv$c2n v1 + cv$c2n v2
-Proof
-  Cases_on`v1` \\ Cases_on`v2` \\ rw[]
-QED
-
-Theorem cv_size'_cv_mk_BN[simp]:
-  cv_size' (cv_mk_BN x y) =
-  cv_add (cv_size' x) (cv_size' y)
-Proof
-  rw[cv_mk_BN_def]
-  \\ TRY (
-    rw[Once cv_size'_def]
-    \\ rw[Once cv_size'_def]
-    \\ Cases_on`x` \\ gs[]
-    \\ rw[Once cv_size'_def, SimpRHS]
-    \\ NO_TAC)
-  \\ rw[Once cv_size'_def]
-  \\ rw[Once cv_size'_def]
-  \\ Cases_on`y` \\ gs[]
-  \\ rw[Once cv_size'_def, SimpRHS]
-  \\ rw[Once cv_size'_def, SimpRHS]
-  \\ rw[Once cv_size'_def]
-QED
-
-Theorem cv_size'_Num[simp]:
-  cv_size' (Num m) = Num 0
-Proof
-  rw[Once cv_size'_def]
-QED
-
-Theorem cv_size'_cv_mk_BS[simp]:
-  cv_size' (cv_mk_BS x y z) =
-  cv_add (cv_add (cv_size' x) (cv_size' z)) (Num 1)
-Proof
-  rw[cv_mk_BS_def]
-  \\ rw[Q.SPEC`Pair x y`cv_size'_def]
-  \\ Cases_on`x` \\ Cases_on`z` \\ gvs[]
-  \\ gvs[Q.SPEC`Pair x y`cv_size'_def]
-QED
-
-Theorem set_byte_160:
-  set_byte a b (w: 160 word) be =
-  let i = byte_index a be in
-       if i =   0 then w2w b        || w && 0xFFFFFFFFFFFFFFFFFFFFFFFFFFFFFFFFFFFFFF00w
-  else if i =   8 then w2w b <<   8 || w && 0xFFFFFFFFFFFFFFFFFFFFFFFFFFFFFFFFFFFF00FFw
-  else if i =  16 then w2w b <<  16 || w && 0xFFFFFFFFFFFFFFFFFFFFFFFFFFFFFFFFFF00FFFFw
-  else if i =  24 then w2w b <<  24 || w && 0xFFFFFFFFFFFFFFFFFFFFFFFFFFFFFFFF00FFFFFFw
-  else if i =  32 then w2w b <<  32 || w && 0xFFFFFFFFFFFFFFFFFFFFFFFFFFFFFF00FFFFFFFFw
-  else if i =  40 then w2w b <<  40 || w && 0xFFFFFFFFFFFFFFFFFFFFFFFFFFFF00FFFFFFFFFFw
-  else if i =  48 then w2w b <<  48 || w && 0xFFFFFFFFFFFFFFFFFFFFFFFFFF00FFFFFFFFFFFFw
-  else if i =  56 then w2w b <<  56 || w && 0xFFFFFFFFFFFFFFFFFFFFFFFF00FFFFFFFFFFFFFFw
-  else if i =  64 then w2w b <<  64 || w && 0xFFFFFFFFFFFFFFFFFFFFFF00FFFFFFFFFFFFFFFFw
-  else if i =  72 then w2w b <<  72 || w && 0xFFFFFFFFFFFFFFFFFFFF00FFFFFFFFFFFFFFFFFFw
-  else if i =  80 then w2w b <<  80 || w && 0xFFFFFFFFFFFFFFFFFF00FFFFFFFFFFFFFFFFFFFFw
-  else if i =  88 then w2w b <<  88 || w && 0xFFFFFFFFFFFFFFFF00FFFFFFFFFFFFFFFFFFFFFFw
-  else if i =  96 then w2w b <<  96 || w && 0xFFFFFFFFFFFFFF00FFFFFFFFFFFFFFFFFFFFFFFFw
-  else if i = 104 then w2w b << 104 || w && 0xFFFFFFFFFFFF00FFFFFFFFFFFFFFFFFFFFFFFFFFw
-  else if i = 112 then w2w b << 112 || w && 0xFFFFFFFFFF00FFFFFFFFFFFFFFFFFFFFFFFFFFFFw
-  else if i = 120 then w2w b << 120 || w && 0xFFFFFFFF00FFFFFFFFFFFFFFFFFFFFFFFFFFFFFFw
-  else if i = 128 then w2w b << 128 || w && 0xFFFFFF00FFFFFFFFFFFFFFFFFFFFFFFFFFFFFFFFw
-  else if i = 136 then w2w b << 136 || w && 0xFFFF00FFFFFFFFFFFFFFFFFFFFFFFFFFFFFFFFFFw
-  else if i = 144 then w2w b << 144 || w && 0xFF00FFFFFFFFFFFFFFFFFFFFFFFFFFFFFFFFFFFFw
-  else if i = 152 then w2w b << 152 || w && 0x00FFFFFFFFFFFFFFFFFFFFFFFFFFFFFFFFFFFFFFw
-  else                 w2w b << 160 || w && 0xFFFFFFFFFFFFFFFFFFFFFFFFFFFFFFFFFFFFFFFFw
-Proof
-  rw_tac std_ss [set_byte_def, word_slice_alt_def]
-  \\ reverse(rpt IF_CASES_TAC)
-  >- (
-    `i = 160`
-    by (
-      qunabbrev_tac`i`
-      \\ full_simp_tac (std_ss ++ boolSimps.LET_ss ++ ARITH_ss) [
-            byte_index_def, EVAL``dimindex(:160)``]
-      \\ `w2n a MOD 20 < 20` by rw[]
-      \\ pop_assum mp_tac
-      \\ qmatch_goalsub_abbrev_tac`z < 20 ⇒ f`
-      \\ simp_tac std_ss [wordsTheory.NUMERAL_LESS_THM]
-      \\ strip_tac \\ gs[Abbr`f`]
-      \\ rw[] \\ gs[] )
-    \\ asm_simp_tac std_ss []
-    \\ simp_tac (srw_ss()) []
-    \\ BBLAST_TAC)
-  \\ asm_simp_tac std_ss []
-  \\ simp_tac (srw_ss()) []
-  \\ BBLAST_TAC
-QED
-
-val () = cv_auto_trans set_byte_160;
-
-val () = cv_auto_trans (INST_TYPE [alpha |-> “:160”] word_of_bytes_def);
-
-(* -- *)
-
-Definition string_to_num_def:
-  string_to_num s = l2n 257 (MAP (SUC o ORD) s)
-End
-
-Definition MAP_CHR_o_PRE_def:
-  MAP_CHR_o_PRE [] acc = REVERSE acc ∧
-  MAP_CHR_o_PRE (x::xs) acc =
-  MAP_CHR_o_PRE xs (CHR(PRE x)::acc)
-End
-
-val MAP_CHR_o_PRE_pre_def = cv_auto_trans_pre MAP_CHR_o_PRE_def;
-
-Theorem MAP_CHR_o_PRE_pre:
-  EVERY ($> 257) v ==>
-  MAP_CHR_o_PRE_pre v acc
-Proof
-  qid_spec_tac`acc` \\ Induct_on`v`
-  \\ rw[Once MAP_CHR_o_PRE_pre_def]
-QED
-
-Theorem MAP_CHR_o_PRE:
-  MAP_CHR_o_PRE ls acc = REVERSE acc ++ (MAP (CHR o PRE) ls)
-Proof
-  qid_spec_tac`acc` \\ Induct_on`ls`
-  \\ rw[MAP_CHR_o_PRE_def]
-QED
-
-Definition num_to_string_def:
-  num_to_string n =
-  if n = 0 then "" else
-  MAP (CHR o PRE) (n2l 257 n)
-End
-
-Theorem string_to_num_to_string:
-  num_to_string (string_to_num s) = s
-Proof
-  simp[num_to_string_def, string_to_num_def, l2n_eq_0]
-  \\ rw[EVERY_MAP]
-  >- (
-    qmatch_assum_abbrev_tac`EVERY P s`
-    \\ `P = K F`
-    by (
-      rw[Abbr`P`, FUN_EQ_THM]
-      \\ DEP_REWRITE_TAC[LESS_MOD]
-      \\ rw[SUC_LT]
-      \\ qexists_tac`256`
-      \\ simp[ORD_BOUND] )
-    \\ Cases_on`s` \\ gvs[] )
-  \\ DEP_REWRITE_TAC[n2l_l2n]
-  \\ simp[l2n_eq_0, EVERY_MAP]
-  \\ DEP_REWRITE_TAC[LOG_l2n]
-  \\ simp[EVERY_MAP, GREATER_DEF, MAP_TAKE, MAP_MAP_o, o_DEF]
-  \\ Cases_on`s = []` \\ gvs[]
-  \\ rw[SUC_LT, EVERY_MEM]
-  \\ qexists_tac`256`
-  \\ simp[ORD_BOUND]
-QED
-
-val () = cv_auto_trans string_to_num_def;
-
-val num_to_string_pre_def = cv_auto_trans_pre (
-  num_to_string_def
- |> REWRITE_RULE[
-      MAP_CHR_o_PRE |> Q.GEN`acc` |> Q.SPEC`[]`
-      |> SIMP_RULE std_ss [APPEND, REVERSE_DEF] |> SYM
-    ] )
-
-Theorem num_to_string_pre[cv_pre]:
-  num_to_string_pre n
-Proof
-  rw[num_to_string_pre_def]
-  \\ irule MAP_CHR_o_PRE_pre
-  \\ irule n2l_BOUND
-  \\ rw[]
-QED
-
 (*
-Theorem num_to_string_inj:
-  (* this is false because of 0 digits *)
-  num_to_string x = num_to_string y ==> x = y
-Proof
-  simp[num_to_string_def]
-  \\ qmatch_goalsub_abbrev_tac`n2l b`
-  \\ pop_assum mp_tac
-  \\ simp[markerTheory.Abbrev_def]
-  \\ qid_spec_tac`y`
-  \\ qid_spec_tac`x`
-  \\ qid_spec_tac`b`
-  \\ ho_match_mp_tac n2l_ind
-  \\ rpt gen_tac \\ strip_tac
-  \\ rpt gen_tac \\ strip_tac
-  \\ gvs[]
-  \\ rw[]
-  >- rw[Once n2l_def]
-  >- rw[Once n2l_def]
-  \\ pop_assum mp_tac
-  \\ rw[Once n2l_def]
-  >- (
-    Cases_on`x` \\ gvs[]
-    \\ qpat_x_assum`n2l _ _ = _`mp_tac
-    \\ rw[Once n2l_def]
-    >- ( Cases_on`x0` \\ gvs[] )
-    \\ rw[Once n2l_def] )
-  \\ pop_assum mp_tac
-  \\ simp[Once n2l_def, SimpRHS]
-  \\ rw[]
-  >- rw[Once n2l_def]
-  \\ gs[]
-  \\ qspec_then`257`mp_tac DIVISION
-  \\ impl_tac >- rw[]
-  \\ disch_then(fn th => qspec_then`x`mp_tac th \\ qspec_then`y`mp_tac th)
-  \\ ntac 2 strip_tac
-  \\ qpat_x_assum`x = _`SUBST1_TAC
-  \\ qpat_x_assum`y = _`SUBST1_TAC
-  \\ qmatch_goalsub_abbrev_tac`xd * _ + xm = yd * _ + ym`
-  \\ `xd = yd ∧ xm = ym` suffices_by rw[]
-  \\ `PRE xm < 256` by (Cases_on`xm` \\ gvs[])
-  \\ `PRE ym < 256` by (Cases_on`ym` \\ gvs[])
-  \\ gs[]
-  \\ Cases_on`xm = 0` >- (
-    gvs[Abbr`xm`, MOD_EQ_0_IFF]
-
-  m``PRE 0``
-
+  plan for cps version:
+  - define the same functions as in evaluate_def, but with an additional
+    continuation argument. make the state argument explicit.
+  - whenever there's a recursive call, make it a tail call and store anything
+    required for the remainder on top of the given continuation
+  - whenever there's a return (or raise), call an "apply" function (these are
+    additional compared to evaluate_def) that applies the continuation to the
+    result (there will be a kind of apply function for each kind of result)
+  - applying a continuation to a result that it doesn't expect is an error: find
+    the results it could expect by looking at where it was created
 *)
 
 Datatype:
-  value
-  = NoneV
-  | BoolV bool
-  | ArrayV bound (value list)
-  | IntV int
-  | StringV num string
-  | BytesV bound (word8 list)
-  | StructV ((identifier, value) alist)
-End
-
-Overload AddressV = “λw: address. BytesV (Fixed 20) (word_to_bytes w T)”
-
-val from_to_value = cv_typeLib.from_to_thm_for “:value”;
-
-Datatype:
-  subscript
-  = IntSubscript int
-  | StrSubscript string
-  | BytesSubscript (word8 list)
-  | AttrSubscript identifier
-End
-
-Datatype:
-  toplevel_value = Value value | HashMap ((subscript, toplevel_value) alist)
-End
-
-Type hmap = “:(subscript, toplevel_value) alist”
-
-Definition default_value_def:
-  default_value env (BaseT (UintT _)) = IntV 0 ∧
-  default_value env (BaseT (IntT _)) = IntV 0 ∧
-  default_value env (TupleT ts) = default_value_tuple env [] ts ∧
-  default_value env (ArrayT _ (Dynamic n)) = ArrayV (Dynamic n) [] ∧
-  default_value env (ArrayT t (Fixed n)) =
-    ArrayV (Fixed n) (REPLICATE n (default_value env t)) ∧
-  default_value env (StructT id) =
-    (let nid = string_to_num id in
-     case FLOOKUP env nid
-       of NONE => StructV []
-        | SOME args => default_value_struct (env \\ nid) [] args) ∧
-  default_value env NoneT = NoneV ∧
-  default_value env (BaseT BoolT) = BoolV F ∧
-  default_value env (BaseT AddressT) = AddressV 0w ∧
-  default_value env (BaseT (StringT n)) = StringV n "" ∧
-  default_value env (BaseT (BytesT (Fixed n))) = BytesV (Fixed n) (REPLICATE n 0w) ∧
-  default_value env (BaseT (BytesT (Dynamic n))) = BytesV (Dynamic n) [] ∧
-  default_value_tuple env acc [] = ArrayV (Fixed (LENGTH acc)) (REVERSE acc) ∧
-  default_value_tuple env acc (t::ts) =
-    default_value_tuple env (default_value env t :: acc) ts ∧
-  default_value_struct env acc [] = StructV (REVERSE acc) ∧
-  default_value_struct env acc ((id,t)::ps) =
-    default_value_struct env ((id,default_value env t)::acc) ps
-Termination
-  WF_REL_TAC ‘inv_image ($< LEX $<) (λx.
-    case x
-      of INL (env, t) => (CARD (FDOM env), type_size t)
-       | INR (INL (env, _, ts)) => (CARD (FDOM env), type1_size ts)
-       | INR (INR (env, _, ps)) => (CARD (FDOM env), type1_size (MAP SND ps)))’
-  \\ rw[type_size_def, FLOOKUP_DEF]
-  \\ disj1_tac
-  \\ CCONTR_TAC
-  \\ fs[]
-End
-
-val () = cv_auto_trans_rec default_value_def (
-  WF_REL_TAC ‘inv_image ($< LEX $<) (λx.
-    case x
-      of INL (env, t) => (cv$c2n $ cv_size' env, cv_size t)
-       | INR (INL (env, _, ts)) => (cv$c2n (cv_size' env), cv_size ts)
-       | INR (INR (env, _, ps)) => (cv$c2n (cv_size' env), cv_size ps))’
-  \\ rw[]
-  \\ TRY(Cases_on`cv_v` \\ gs[] \\ NO_TAC)
-  \\ TRY(Cases_on`cv_v` \\ gs[]
-         \\ qmatch_asmsub_rename_tac`cv_ispair cv_v`
-         \\ Cases_on`cv_v` \\ gs[] \\ NO_TAC)
-  \\ TRY(Cases_on`cv_v` \\ gs[]
-         \\ qmatch_goalsub_rename_tac`cv_fst cv_v`
-         \\ Cases_on`cv_v` \\ gs[] \\ NO_TAC)
-  \\ disj1_tac
-  \\ pop_assum mp_tac
-  \\ qmatch_goalsub_abbrev_tac`cv_lookup ck`
-  \\ `cv_ispair ck = Num 0`
-  by (
-    rw[Abbr`ck`, definition"cv_string_to_num_def"]
-    \\ rw[Once keccakTheory.cv_l2n_def]
-    \\ rw[cv_ispair_cv_add] )
-  \\ pop_assum mp_tac
-  \\ qid_spec_tac`cv_env`
-  \\ qid_spec_tac`ck`
-  \\ rpt (pop_assum kall_tac)
-  \\ ho_match_mp_tac cv_stdTheory.cv_delete_ind
-  \\ rpt gen_tac \\ strip_tac
-  \\ simp[Once cv_lookup_def]
-  \\ IF_CASES_TAC \\ gs[]
-  \\ strip_tac \\ gs[]
-  \\ reverse(IF_CASES_TAC \\ gs[])
-  >- (
-    Cases_on`ck` \\ gs[]
-    \\ IF_CASES_TAC \\ gs[]
-    \\ Cases_on`cv_env` \\ gs[]
-    \\ Cases_on`0 < m` \\ gs[]
-    \\ simp[Once cv_delete_def]
-    \\ rw[Once cv_stdTheory.cv_size'_def]
-    \\ rw[Once cv_stdTheory.cv_size'_def] )
-  \\ Cases_on`cv_env` \\ gs[]
-  \\ Cases_on`ck` \\ gs[]
-  \\ strip_tac
-  \\ simp[Once cv_delete_def]
-  \\ Cases_on`g` \\ gs[]
-  \\ Cases_on`m=0` \\ gs[]
-  >- (
-    rw[] \\ gs[]
-    \\ rw[Once cv_stdTheory.cv_size'_def]
-    \\ rw[Once cv_stdTheory.cv_size'_def, SimpR``prim_rec$<``]
-    \\ rw[] )
-  \\ simp[Once cv_stdTheory.cv_size'_def, SimpR``prim_rec$<``]
-  \\ qmatch_goalsub_rename_tac`2 < p`
-  \\ Cases_on`p=0` \\ gs[]
-  \\ Cases_on`p=1` \\ gs[]
-  \\ Cases_on`p=2` \\ gvs[]
-  >- (IF_CASES_TAC \\ gs[cv_size'_cv_mk_BN])
-  \\ IF_CASES_TAC \\ gs[]
-);
-
-(*
-We don't use this directly to support cv which prefers num keys
-Type scope = “:identifier |-> value”;
-*)
-Type scope = “:num |-> value”;
-
-val from_to_value_thm = cv_typeLib.from_to_thm_for “:value”;
-val from_value = from_to_value_thm |> concl |> rator |> rand
-val to_value = from_to_value_thm |> concl |> rand
-
-(*
-Definition from_scope_def:
-  from_scope env = from_fmap ^from_value (env f_o num_to_string)
-End
-
-Definition to_scope_def:
-  to_scope cv = to_fmap ^to_value cv f_o string_to_num
-End
-
-Theorem from_to_scope[cv_from_to]:
-  from_to from_scope to_scope
-Proof
-  mp_tac $ MATCH_MP from_to_fmap from_to_value_thm
-  \\ rw[from_to_def, from_scope_def, to_scope_def]
-  \\ DEP_REWRITE_TAC[f_o_ASSOC]
-  \\ rw[EQ_IMP_THM]
-  >- cheat
-  >- metis_tac[string_to_num_to_string]
-  \\ irule (iffLR fmap_EQ_THM)
-  \\ DEP_REWRITE_TAC[FDOM_f_o]
-  \\ simp[o_DEF, string_to_num_to_string]
-  \\ rw[]
-  \\ DEP_REWRITE_TAC[FAPPLY_f_o]
-  \\ simp[]
-QED
-*)
-
-Definition lookup_scopes_def:
-  lookup_scopes id [] = NONE ∧
-  lookup_scopes id ((env: scope)::rest) =
-  case FLOOKUP env id of NONE =>
-    lookup_scopes id rest
-  | SOME v => SOME v
-End
-
-Datatype:
-  expr_continuation
-  = StartExpr expr
-  (*
-  | NamedExprK1 expr_continuation expr
-  | NamedExprK2 value expr_continuation
-  *)
-  | IfExpK expr_continuation expr expr
-  | ArrayLitK bound (value list) expr_continuation (expr list)
-  | SubscriptK1 expr_continuation expr
-  | SubscriptK2 value expr_continuation
-  | SubscriptMapK hmap expr_continuation
-  | AttributeK expr_continuation identifier
-  | BuiltinK builtin (value list) expr_continuation (expr list)
-  | CallK call_target (value list) expr_continuation (expr list)
-  | LiftCall call_target (value list) expr_continuation
-  | DoneExpr value
-  | DoneExprMap hmap
-  | ReturnExpr
-  | ErrorExpr string
-End
-
-Type containing_scope = “: scope list # scope # scope list”;
-
-Datatype:
-  location
-  = ScopedVar containing_scope identifier
-  | Global identifier
-End
-
-Datatype:
-  assignment_value
-  = BaseTargetV location (subscript list)
-  | TupleTargetV (assignment_value list)
-End
-
-Datatype:
-  base_tgt_continuation
-  = StartBaseTgt base_assignment_target
-  | SubscriptTargetK1 base_tgt_continuation expr
-  | SubscriptTargetK2 location (subscript list) expr_continuation
-  | AttributeTargetK base_tgt_continuation identifier
-  | LiftCallBaseTgt call_target (value list) base_tgt_continuation
-  | DoneBaseTgt location (subscript list)
-  | ErrorBaseTgt string
-End
-
-Datatype:
-  tgt_continuation
-  = StartTgt assignment_target
-  | TupleTargetK (assignment_value list) tgt_continuation (assignment_target list)
-  | BaseTargetK base_tgt_continuation
-  | LiftCallTgt call_target (value list) tgt_continuation
-  | DoneTgt assignment_value
-  | ErrorTgt string
-End
-
-Datatype:
-  exception
-  = RaiseException string
-  | AssertException string
-  | Error string
-  | ExternalReturn value
-End
-
-Datatype:
-  stmt_continuation
-  = StartK stmt
-  | ExprK expr_continuation
-  | IfK expr_continuation (stmt list) (stmt list)
-  | AssertK expr_continuation string
-  | ReturnSomeK expr_continuation
-  | AssignK1 tgt_continuation expr
-  | AssignK2 assignment_value expr_continuation
-  | AugAssignK1 base_tgt_continuation binop expr
-  | AugAssignK2 location (subscript list) binop expr_continuation
-  | AnnAssignK identifier type expr_continuation
-  | ForK identifier type expr_continuation num (stmt list)
+  eval_continuation
+  = ReturnK eval_continuation
+  | AssertK string eval_continuation
+  | AnnAssignK identifier eval_continuation
+  | AssignK expr eval_continuation
+  | AssignK1 assignment_value eval_continuation
+  | AugAssignK binop expr eval_continuation
+  | AugAssignK1 base_target_value binop eval_continuation
+  | IfK (stmt list) (stmt list) eval_continuation
+  | IfK1 toplevel_value (stmt list) (stmt list) eval_continuation
+  | IfK2 eval_continuation
+  | ForK identifier num (stmt list) eval_continuation
+  | ForK1 num (stmt list) (value list) eval_continuation
+  | ExprK eval_continuation
+  | StmtsK (stmt list) eval_continuation
+  | BaseTargetK eval_continuation
+  | TupleTargetK eval_continuation
+  | TargetsK (assignment_target list) eval_continuation
+  | TargetsK1 assignment_value eval_continuation
+  | AttributeTargetK identifier eval_continuation
+  | SubscriptTargetK expr eval_continuation
+  | SubscriptTargetK1 base_target_value eval_continuation
+  | IfExpK expr expr eval_continuation
+  | ArrayLitK bound eval_continuation
+  | SubscriptK expr eval_continuation
+  | SubscriptK1 toplevel_value eval_continuation
+  | AttributeK identifier eval_continuation
+  | BuiltinK builtin eval_continuation
+  | CallSendK eval_continuation
+  | IntCallK identifier ((identifier # type) list) (stmt list) eval_continuation
+  | IntCallK1 (scope list) eval_continuation
+  | ExprsK (expr list) eval_continuation
+  | ExprsK1 value eval_continuation
   | DoneK
-  | ExceptionK exception
-End
-
-Definition evaluate_literal_def:
-  evaluate_literal (BoolL b)   = BoolV b ∧
-  evaluate_literal (StringL n s) = StringV n s ∧
-  evaluate_literal (BytesL b bs) = BytesV b bs ∧
-  evaluate_literal (IntL i)    = IntV i
-End
-
-val () = cv_auto_trans evaluate_literal_def;
-
-Definition evaluate_binop_def:
-  evaluate_binop (Add:binop) (IntV i1) (IntV i2) = DoneExpr (IntV (i1 + i2)) ∧
-  evaluate_binop Sub (IntV i1) (IntV i2) = DoneExpr (IntV (i1 - i2)) ∧
-  evaluate_binop Mul (IntV i1) (IntV i2) = DoneExpr (IntV (i1 * i2)) ∧
-  evaluate_binop _ _ _ = ErrorExpr "binop"
-End
-
-val () = cv_auto_trans evaluate_binop_def;
-
-Definition evaluate_builtin_def:
-  evaluate_builtin _ Len [BytesV _ ls] = DoneExpr (IntV &(LENGTH ls)) ∧
-  evaluate_builtin _ Len [StringV _ ls] = DoneExpr (IntV &(LENGTH ls)) ∧
-  evaluate_builtin _ Len [ArrayV _ ls] = DoneExpr (IntV &(LENGTH ls)) ∧
-  evaluate_builtin _ Eq [StringV _ s1; StringV _ s2] = DoneExpr (BoolV (s1 = s2)) ∧
-  evaluate_builtin _ Eq [BytesV _ s1; BytesV _ s2] = DoneExpr (BoolV (s1 = s2)) ∧
-  evaluate_builtin _ Eq [BoolV b1; BoolV b2] = DoneExpr (BoolV (b1 = b2)) ∧
-  evaluate_builtin _ Eq  [IntV i1; IntV i2] = DoneExpr (BoolV (i1 = i2)) ∧
-  evaluate_builtin _ Lt  [IntV i1; IntV i2] = DoneExpr (BoolV (i1 < i2)) ∧
-  evaluate_builtin _ Not [BoolV b] = DoneExpr (BoolV (¬b)) ∧
-  evaluate_builtin _ (Bop bop) [v1; v2] = evaluate_binop bop v1 v2 ∧
-  evaluate_builtin bal (Acc Balance) [BytesV _ bs] =
-    (case ALOOKUP bal (word_of_bytes T (0w:address) bs) of
-          SOME n => DoneExpr (IntV &n)
-        | NONE => ErrorExpr "missing balance") ∧
-  evaluate_builtin _ _ _ = ErrorExpr "builtin"
-End
-
-val () = cv_auto_trans evaluate_builtin_def;
-
-Definition extract_elements_def:
-  extract_elements (ArrayV _ vs) = SOME vs ∧
-  extract_elements _ = NONE
-End
-
-val () = cv_auto_trans extract_elements_def;
-
-Definition replace_elements_def:
-  replace_elements (ArrayV b _) vs = SOME (ArrayV b vs) ∧
-  replace_elements _ _ = NONE
-End
-
-val () = cv_auto_trans replace_elements_def;
-
-Definition integer_index_def:
-  integer_index vs i =
-   if Num i < LENGTH vs then
-     SOME $ if 0 ≤ i then Num i else LENGTH vs - Num i
-   else NONE
-End
-
-val () = cv_auto_trans integer_index_def;
-
-Definition evaluate_subscript_def:
-  evaluate_subscript av (IntV i) =
-  (case extract_elements av of SOME vs =>
-    (case integer_index vs i of SOME j => DoneExpr (EL j vs)
-     | _ => ErrorExpr "integer_index")
-   | _ => ErrorExpr "extract_elements") ∧
-  evaluate_subscript _ _ = ErrorExpr "evaluate_subscript"
-End
-
-val evaluate_subscript_pre_def = cv_auto_trans_pre evaluate_subscript_def;
-
-Theorem evaluate_subscript_pre[cv_pre]:
-  evaluate_subscript_pre av v
-Proof
-  rw[evaluate_subscript_pre_def, integer_index_def]
-  \\ rw[]
-  \\ qmatch_asmsub_rename_tac`0i ≤ v0`
-  \\ Cases_on`v0` \\ gs[]
-QED
-
-Definition evaluate_attribute_def:
-  evaluate_attribute (StructV kvs) id =
-  (case ALOOKUP kvs id of SOME v => DoneExpr v
-   | _ => ErrorExpr "attribute") ∧
-  evaluate_attribute _ _ = ErrorExpr "evaluate_attribute"
-End
-
-val () = cv_auto_trans evaluate_attribute_def;
-
-Definition compatible_bound_def:
-  compatible_bound (Fixed n) m = (n = m) ∧
-  compatible_bound (Dynamic n) m = (m ≤ n)
-End
-
-val () = cv_auto_trans compatible_bound_def;
-
-Definition builtin_args_length_ok_def:
-  builtin_args_length_ok Len n = (n = 1n) ∧
-  builtin_args_length_ok Not n = (n = 1) ∧
-  builtin_args_length_ok Eq n = (n = 2) ∧
-  builtin_args_length_ok Lt n = (n = 2) ∧
-  builtin_args_length_ok (Bop _) n = (n = 2) ∧
-  builtin_args_length_ok (Msg _) n = (n = 0) ∧
-  builtin_args_length_ok (Acc _) n = (n = 1)
-End
-
-val () = cv_auto_trans builtin_args_length_ok_def;
-
-Datatype:
-  transaction = <|
-    sender: address
-  ; target: address
-  ; function_name: identifier
-  ; args: value list
-  ; value: num
-  |>
-End
-
-Definition value_to_key_def:
-  value_to_key (IntV i) = SOME $ IntSubscript i ∧
-  value_to_key (StringV _ s) = SOME $ StrSubscript s ∧
-  value_to_key (BytesV _ bs) = SOME $ BytesSubscript bs ∧
-  value_to_key _ = NONE
-End
-
-val () = cv_auto_trans value_to_key_def;
-
-Datatype:
-  expr_ctxt = <|
-    tx: transaction
-  ; gbs: num |-> toplevel_value
-  ; env: scope list
-  ; bal: (address, num) alist
-  |>
-End
-
-Definition step_expr_def:
-  step_expr ctx (StartExpr (Literal l)) =
-    DoneExpr (evaluate_literal l) ∧
-  step_expr ctx (StartExpr (ArrayLit b [])) = (
-    if compatible_bound b 0
-    then DoneExpr (ArrayV b [])
-    else ErrorExpr "ArrayLit [] bound" ) ∧
-  step_expr ctx (StartExpr (ArrayLit b (e::es))) = (
-    if compatible_bound b (LENGTH (e::es))
-    then ArrayLitK b [] (StartExpr e) es
-    else ErrorExpr "ArrayLit :: bound" ) ∧
-  step_expr ctx (StartExpr (Name id)) =
-    (case lookup_scopes (string_to_num id) ctx.env
-     of SOME v => DoneExpr v
-      | _ => ErrorExpr "lookup_scopes") ∧
-  step_expr ctx (StartExpr (TopLevelName id)) =
-    (case FLOOKUP ctx.gbs (string_to_num id)
-     of SOME (Value v) => DoneExpr v
-      | SOME (HashMap ls) => DoneExprMap ls
-      | _ => ErrorExpr "lookup gbs") ∧
-  step_expr ctx (StartExpr (Subscript e1 e2)) =
-    SubscriptK1 (StartExpr e1) e2 ∧
-  step_expr ctx (StartExpr (Attribute e id)) =
-    AttributeK (StartExpr e) id ∧
-  step_expr ctx (StartExpr (IfExp e1 e2 e3)) =
-    IfExpK (StartExpr e1) e2 e3 ∧
-  step_expr ctx (StartExpr (Builtin (Msg Sender) [])) =
-    DoneExpr (AddressV ctx.tx.sender) ∧
-  step_expr ctx (StartExpr (Builtin (Msg SelfAddr) [])) =
-    DoneExpr (AddressV ctx.tx.target) ∧
-  step_expr ctx (StartExpr (Builtin (Msg ValueSent) [])) =
-    DoneExpr (IntV &ctx.tx.value) ∧
-  step_expr ctx (StartExpr (Builtin bt [])) =
-    ErrorExpr "builtin no args" ∧
-  step_expr ctx (StartExpr (Builtin bt (e::es))) = (
-    if builtin_args_length_ok bt (LENGTH (e::es))
-    then BuiltinK bt [] (StartExpr e) es
-    else ErrorExpr "builtin args length" ) ∧
-  step_expr ctx (StartExpr (Call id [])) =
-    LiftCall id [] ReturnExpr ∧
-  step_expr ctx (StartExpr (Call id (e::es))) =
-    CallK id [] (StartExpr e) es ∧
-  (*
-  step_expr gbs env (NamedExprK1 k e) =
-    (case step_expr gbs env k
-     of ErrorExpr => ErrorExpr
-      | DoneExpr v => NamedExprK2 v (StartExpr e)
-      | LiftCall id vs k => LiftCall id vs (NamedExprK1 k e)
-      | k => NamedExprK1 k e) ∧
-  step_expr gbs env (NamedExprK2 v1 k) =
-    (case step_expr gbs env k
-     of ErrorExpr => ErrorExpr
-      | DoneExpr v2 =>
-  *)
-  step_expr ctx (IfExpK k e2 e3) =
-  (case step_expr ctx k
-   of ErrorExpr msg => ErrorExpr msg
-    | DoneExprMap _ => ErrorExpr "IfExpK Map"
-    | DoneExpr v1 => (case v1 of BoolV b => StartExpr (if b then e2 else e3)
-                               | _ => ErrorExpr "IfExpK value")
-    | LiftCall id vs k => LiftCall id vs (IfExpK k e2 e3)
-    | k => IfExpK k e2 e3) ∧
-  step_expr ctx (ArrayLitK b vs k es) =
-  (case step_expr ctx k
-   of ErrorExpr msg => ErrorExpr msg
-    | DoneExprMap _ => ErrorExpr "ArrayLitK Map"
-    | DoneExpr v =>
-        (case es of (e::es) => ArrayLitK b (SNOC v vs) (StartExpr e) es
-                  | [] => DoneExpr (ArrayV b (SNOC v vs)))
-    | LiftCall id as k => LiftCall id as (ArrayLitK b vs k es)
-    | k => ArrayLitK b vs k es) ∧
-  step_expr ctx (SubscriptK1 k e) =
-  (case step_expr ctx k
-   of ErrorExpr msg => ErrorExpr msg
-    | DoneExpr v => SubscriptK2 v (StartExpr e)
-    | DoneExprMap hm => SubscriptMapK hm (StartExpr e)
-    | LiftCall id vs k => LiftCall id vs (SubscriptK1 k e)
-    | k => SubscriptK1 k e) ∧
-  step_expr ctx (SubscriptK2 v1 k) =
-  (case step_expr ctx k
-   of ErrorExpr msg => ErrorExpr msg
-    | DoneExprMap _ => ErrorExpr "SubscriptK2 Map"
-    | DoneExpr v2 => evaluate_subscript v1 v2
-    | LiftCall id vs k => LiftCall id vs (SubscriptK2 v1 k)
-    | k => SubscriptK2 v1 k) ∧
-  step_expr ctx (SubscriptMapK hm k) =
-  (case step_expr ctx k
-   of ErrorExpr msg => ErrorExpr msg
-    | DoneExprMap _ => ErrorExpr "SubscriptMapK Map"
-    | DoneExpr v2 =>
-        (case value_to_key v2 of SOME k =>
-          (case ALOOKUP hm k of
-           SOME (Value v) => DoneExpr v
-           (* TODO: more hashmaps *)
-           | _ => ErrorExpr "SubscriptMapK lookup")
-         | _ => ErrorExpr "value_to_key")
-    | LiftCall id vs k => LiftCall id vs (SubscriptMapK hm k)
-    | k => SubscriptMapK hm k) ∧
-  step_expr ctx (AttributeK k id) =
-  (case step_expr ctx k
-   of ErrorExpr msg => ErrorExpr msg
-    | DoneExprMap _ => ErrorExpr "AttributeK Map"
-    | DoneExpr v => evaluate_attribute v id
-    | LiftCall fn vs k => LiftCall fn vs (AttributeK k id)
-    | k => AttributeK k id) ∧
-  step_expr ctx (BuiltinK bt vs k es) =
-  (case step_expr ctx k
-   of ErrorExpr msg => ErrorExpr msg
-    | DoneExprMap _ => ErrorExpr "BuiltinK Map"
-    | DoneExpr v1 =>
-        (let vs = SNOC v1 vs in
-         case es of (e::es) =>
-           BuiltinK bt vs (StartExpr e) es
-          | [] => evaluate_builtin ctx.bal bt vs)
-    | LiftCall id ws k => LiftCall id ws (BuiltinK bt vs k es)
-    | k => BuiltinK bt vs k es) ∧
-  step_expr ctx (CallK id vs k es) =
-  (case step_expr ctx k
-   of ErrorExpr msg => ErrorExpr msg
-    | DoneExprMap _ => ErrorExpr "CallK Map"
-    | DoneExpr v =>
-        (let vs = SNOC v vs in
-         case es of (e::es) => CallK id vs (StartExpr e) es
-                  | [] => LiftCall id vs ReturnExpr)
-    | LiftCall id ws k => LiftCall id ws (CallK id vs k es)
-    | k => CallK id vs k es) ∧
-  step_expr ctx (LiftCall id vs k) = LiftCall id vs k ∧
-  step_expr ctx (DoneExpr v) = DoneExpr v ∧
-  step_expr ctx (DoneExprMap ls) = DoneExprMap ls ∧
-  step_expr ctx ReturnExpr = ReturnExpr ∧
-  step_expr ctx (ErrorExpr msg) = ErrorExpr msg
-End
-
-val () = cv_auto_trans step_expr_def;
-
-Datatype:
-  loop_info = <|
-    loop_var: (* identifier *) num
-  ; loop_first_stmt: stmt
-  ; loop_rest_stmts: stmt list
-  ; remaining_values: value list
-  |>
 End
 
 Datatype:
-  function_or_loop = Fn identifier | Loop loop_info
+  apply_base_continuation
+  = Apply
+  | ApplyExc exception
+  | ApplyTarget assignment_value
+  | ApplyTargets (assignment_value list)
+  | ApplyBaseTarget base_target_value
+  | ApplyTv toplevel_value
+  | ApplyVal value
+  | ApplyVals (value list)
 End
 
 Datatype:
-  function_context =
-  <| scopes: scope list
-   ; current_stmt: stmt_continuation
-   ; remaining_stmts: stmt list
-   ; name: function_or_loop
-   |>
+  apply_continuation
+  = AK evaluation_context apply_base_continuation
+       evaluation_state eval_continuation
 End
 
-Definition initial_function_context_def:
-  initial_function_context fn args ss = <|
-    scopes := [args]
-  ; current_stmt := (case ss of s::_ => StartK s
-                        | _ => ExceptionK (Error "initial_function_context"))
-  ; remaining_stmts := TL ss
-  ; name := Fn fn
-  |>
+Definition liftk_def:
+  liftk cx a (INL x, st) = AK cx (a x) (st:evaluation_state) ∧
+  liftk cx a (INR (ex:exception), st) = AK cx (ApplyExc ex) st
 End
 
-val () = cv_auto_trans initial_function_context_def;
+val liftk1 = oneline liftk_def;
 
-(* TODO: assumes unique identifiers, but should check? *)
-Definition initial_globals_def:
-  initial_globals env [] = FEMPTY ∧
-  initial_globals env (VariableDecl _ Storage id typ :: ts) =
-  initial_globals env ts |+ (string_to_num id, Value $ default_value env typ) ∧
-  initial_globals env (VariableDecl _ Transient id typ :: ts) =
-  initial_globals env ts |+ (string_to_num id, Value $ default_value env typ) ∧
-  (* TODO: handle Constants and  Immutables *)
-  initial_globals env (HashMapDecl _ id kt vt :: ts) =
-  initial_globals env ts |+ (string_to_num id, HashMap []) ∧
-  initial_globals env (t :: ts) = initial_globals env ts
+Definition no_recursion_def:
+  no_recursion (fn:identifier) stk ⇔ ¬MEM fn stk
 End
 
-val () = cv_auto_trans initial_globals_def;
+val () = cv_auto_trans no_recursion_def;
 
-Datatype:
-  contract = <|
-    src: toplevel list
-  ; globals: (* identifier *) num |-> toplevel_value
-  |>
-End
-
-Datatype:
-  execution_context = <|
-    current_fc : function_context
-  ; call_stack : function_context list
-  ; current_contract: contract
-  ; current_transaction: transaction
-  ; current_balances: (address, num) alist
-  |>
-End
-
-Datatype:
-  machine_state = <|
-    contracts: (address, contract) alist (* TODO: use a function (sptree under cv) *)
-  ; balances: (address, num) alist (* TODO: similarly *)
-  |>
-End
-
-Definition initial_machine_state_def:
-  initial_machine_state = <| contracts := []; balances := [] |>
-End
-
-val () = cv_auto_trans initial_machine_state_def;
-
-Definition type_env_def:
-  type_env [] = FEMPTY ∧
-  type_env (StructDef id args :: ts) =
-    type_env ts |+ (string_to_num id, args) ∧
-  type_env (_ :: ts) = type_env ts
-End
-
-val () = cv_auto_trans type_env_def;
-
-Definition initial_execution_context_def:
-  initial_execution_context t c b fc = <|
-    current_fc := fc
-  ; call_stack := []
-  ; current_contract := c
-  ; current_transaction := t
-  ; current_balances := b
-  |>
-End
-
-val () = cv_auto_trans initial_execution_context_def;
-
-Definition raise_def:
-  raise err ctx = ctx with current_fc updated_by
-    (λfc. fc with current_stmt := ExceptionK err)
-End
-
-val () = cv_auto_trans raise_def;
-
-Definition push_scope_def:
-  push_scope ctx =
-    ctx with current_fc updated_by (λfc. fc with scopes updated_by CONS FEMPTY)
-End
-
-val () = cv_auto_trans push_scope_def;
-
-Definition pop_scope_def:
-  pop_scope ctx =
-  case ctx.current_fc.scopes
-    of [] => raise (Error "pop_scope") ctx
-     | (_::rest) => ctx with current_fc updated_by (λfc. fc with scopes := rest)
-End
-
-val () = cv_auto_trans pop_scope_def;
-
-Definition new_variable_def:
-  new_variable id typ ctx =
-  let tenv = type_env ctx.current_contract.src in
-  case ctx.current_fc.scopes
-    of [] => raise (Error "new_variable") ctx
-     | env::rest =>
-         if id ∈ FDOM env then raise (Error "var exists") ctx
-         else ctx with current_fc updated_by
-           (λfc. fc with scopes := (env |+ (id, default_value tenv typ))::rest)
-End
-
-val () = cv_auto_trans (REWRITE_RULE[TO_FLOOKUP]new_variable_def);
-
-Definition find_containing_scope_def:
-  find_containing_scope id [] = NONE : containing_scope option ∧
-  find_containing_scope id (env::rest) =
-  if id ∈ FDOM env then SOME ([], env, rest)
-  else OPTION_MAP (λ(p,q). (env::p, q)) (find_containing_scope id rest)
-End
-
-val () = cv_auto_trans (REWRITE_RULE[TO_FLOOKUP]find_containing_scope_def);
-
-Definition step_base_target_def:
-  step_base_target ctx (StartBaseTgt (NameTarget id)) =
-    (case find_containing_scope (string_to_num id) ctx.env
-     of SOME cs => DoneBaseTgt (ScopedVar cs id) []
-      | _ => ErrorBaseTgt "step_base_target find_containing_scope" ) ∧
-  step_base_target ctx (StartBaseTgt (TopLevelNameTarget id)) =
-    DoneBaseTgt (Global id) [] ∧
-  step_base_target ctx (StartBaseTgt (SubscriptTarget t e)) =
-    SubscriptTargetK1 (StartBaseTgt t) e ∧
-  step_base_target cxt (StartBaseTgt (AttributeTarget t id)) =
-    AttributeTargetK (StartBaseTgt t) id ∧
-  step_base_target ctx (SubscriptTargetK1 k e) =
-    (case step_base_target ctx k of
-     | DoneBaseTgt l s => SubscriptTargetK2 l s (StartExpr e)
-     | LiftCallBaseTgt fn vs k => LiftCallBaseTgt fn vs (SubscriptTargetK1 k e)
-     | ErrorBaseTgt msg => ErrorBaseTgt msg
-     | k => SubscriptTargetK1 k e) ∧
-  step_base_target ctx (SubscriptTargetK2 l s k) =
-   (case step_expr ctx k
-    of DoneExpr v => (case value_to_key v of SOME k => DoneBaseTgt l (k::s)
-                      | _ => ErrorBaseTgt "SubscriptTargetK2 value_to_key")
-     | DoneExprMap _ => ErrorBaseTgt "SubscriptTargetK2 Map"
-     | ErrorExpr msg => ErrorBaseTgt msg
-     | LiftCall fn vs k => LiftCallBaseTgt fn vs (SubscriptTargetK2 l s k)
-     | k => SubscriptTargetK2 l s k) ∧
-  step_base_target ctx (AttributeTargetK k id) =
-  (case step_base_target ctx k
-   of ErrorBaseTgt msg => ErrorBaseTgt msg
-    | DoneBaseTgt l s => DoneBaseTgt l ((AttrSubscript id)::s)
-    | LiftCallBaseTgt fn vs k => LiftCallBaseTgt fn vs (AttributeTargetK k id)
-    | k => AttributeTargetK k id) ∧
-  step_base_target ctx (LiftCallBaseTgt fn vs k) = LiftCallBaseTgt fn vs k ∧
-  step_base_target ctx (DoneBaseTgt l s) = DoneBaseTgt l s ∧
-  step_base_target ctx (ErrorBaseTgt msg) = ErrorBaseTgt msg
-End
-
-val () = cv_auto_trans step_base_target_def;
-
-Definition step_target_def:
-  step_target ctx (StartTgt (BaseTarget b)) =
-    BaseTargetK (StartBaseTgt b) ∧
-  step_target ctx (StartTgt (TupleTarget [])) =
-    DoneTgt (TupleTargetV []) ∧
-  step_target ctx (StartTgt (TupleTarget (t::ts))) =
-    TupleTargetK [] (StartTgt t) ts ∧
-  step_target ctx (TupleTargetK vs k ts) =
-  (case step_target ctx k
-   of DoneTgt v =>
-     (case ts of [] => DoneTgt (TupleTargetV (SNOC v vs))
-               | (t::ts) => TupleTargetK (SNOC v vs) (StartTgt t) ts)
-    | LiftCallTgt fn as k =>
-        LiftCallTgt fn as (TupleTargetK vs k ts)
-    | ErrorTgt msg => ErrorTgt msg
-    | k => TupleTargetK vs k ts) ∧
-  step_target ctx (BaseTargetK k) =
-  (case step_base_target ctx k
-   of DoneBaseTgt l s => DoneTgt $ BaseTargetV l s
-    | LiftCallBaseTgt fn vs k => LiftCallTgt fn vs (BaseTargetK k)
-    | ErrorBaseTgt msg => ErrorTgt msg
-    | k => BaseTargetK k) ∧
-  step_target ctx (LiftCallTgt fn vs k) = LiftCallTgt fn vs k ∧
-  step_target ctx (DoneTgt v) = DoneTgt v ∧
-  step_target ctx (ErrorTgt msg) = ErrorTgt msg
-End
-
-val () = cv_auto_trans step_target_def;
-
-Definition set_variable_def:
-  set_variable id v ctx =
-  case find_containing_scope id ctx.current_fc.scopes
-    of NONE => raise (Error "find_containing_scope") ctx
-     | SOME (pre, env, rest) =>
-         (* check that v has same type as current value here ? *)
-         ctx with current_fc updated_by
-           (λfc. fc with scopes := pre ++ (env |+ (id, v))::rest)
-End
-
-val () = cv_auto_trans set_variable_def;
-
-Datatype:
-  assign_operation = Replace value | Update binop value
-End
-
-Definition assign_subscripts_def:
-  assign_subscripts a [] (Replace v) = SOME v ∧
-  assign_subscripts a [] (Update bop v) =
-  (case evaluate_binop bop a v
-     of DoneExpr w => SOME w
-      | _ => NONE) ∧
-  assign_subscripts a ((IntSubscript i)::is) ao =
-  (case extract_elements a of SOME vs =>
-   (case integer_index vs i of SOME j =>
-    (case assign_subscripts (EL j vs) is ao of SOME vj =>
-       replace_elements a (TAKE j vs ++ [vj] ++ DROP (SUC j) vs)
-     | _ => NONE)
-    | _ => NONE)
-   | _ => NONE) ∧
-  assign_subscripts _ _ _ = NONE (* TODO: handle AttrSubscript *)
-End
-
-val assign_subscripts_pre_def = cv_auto_trans_pre assign_subscripts_def;
-
-Theorem assign_subscripts_pre[cv_pre]:
-  !a b c. assign_subscripts_pre a b c
-Proof
-  ho_match_mp_tac assign_subscripts_ind
-  \\ rw[Once assign_subscripts_pre_def]
-  \\ rw[Once assign_subscripts_pre_def]
-  \\ gvs[integer_index_def] \\ rw[]
-  \\ qmatch_asmsub_rename_tac`0i ≤ v0`
-  \\ Cases_on`v0` \\ gs[]
-QED
-
-Definition assign_hashmap_def:
-  assign_hashmap hm [] _ = NONE ∧
-  assign_hashmap hm [k] (Replace v) =
-    SOME $ (k,Value v)::(ADELKEY k hm) ∧
-  assign_hashmap hm [k] (Update bop v2) =
-  (case ALOOKUP hm k of SOME (Value v1) =>
-     (case evaluate_binop bop v1 v2 of DoneExpr w =>
-        SOME $ (k,Value w)::(ADELKEY k hm) | _ => NONE)
-   | _ => NONE) ∧
-  assign_hashmap hm (k::ks) ao =
-  (case ALOOKUP hm k of SOME (HashMap hm') =>
-    (case assign_hashmap hm' ks ao of
-     | SOME hm' => SOME $ (k, HashMap hm') :: (ADELKEY k hm)
-     | _ => NONE)
-    | _ => NONE)
-End
-
-val () = cv_auto_trans assign_hashmap_def;
-
-Definition assign_target_def:
-  assign_target (BaseTargetV (ScopedVar (pre,env,rest) id) is) ao ctx =
-    (let nid = string_to_num id in
-    (case FLOOKUP env nid of SOME a =>
-     (case assign_subscripts a is ao of SOME a' =>
-        ctx with current_fc updated_by
-          (λfc. fc with scopes := pre ++ (env |+ (nid, a'))::rest)
-      | _ => raise (Error "assign_subscripts ScopedVar") ctx)
-     | _ => raise (Error "assign_target lookup") ctx)) ∧
-  assign_target (BaseTargetV (Global id) is) ao ctx =
-  (let nid = string_to_num id in
-  (case FLOOKUP ctx.current_contract.globals nid
-   of SOME (Value a) =>
-     (case assign_subscripts a is ao of SOME a' =>
-       ctx with current_contract updated_by
-         (λcc. cc with globals := cc.globals |+ (nid, Value a'))
-      | _ => raise (Error "assign_subscripts Global") ctx)
-   | SOME (HashMap hm) =>
-     (case assign_hashmap hm is ao of SOME hm' =>
-       ctx with current_contract updated_by
-         (λcc. cc with globals := cc.globals |+ (nid, HashMap hm'))
-      | _ => raise (Error "assign_hashmap Global") ctx)
-   | _ => raise (Error "assign_target globals lookup") ctx)) ∧
-  assign_target _ _ ctx = raise (Error "TODO: TupleTargetV") ctx
-End
-
-val () = cv_auto_trans assign_target_def;
-
-(* TODO: check types? *)
-Definition bind_arguments_def:
-  bind_arguments ([]: argument list) [] = SOME (FEMPTY: scope) ∧
-  bind_arguments ((id, typ)::params) (v::vs) =
-    OPTION_MAP (λm. m |+ (string_to_num id, v)) (bind_arguments params vs) ∧
-  bind_arguments _ _ = NONE
-End
-
-val () = cv_auto_trans bind_arguments_def;
-
-Definition is_ArrayT_def[simp]:
-  is_ArrayT (ArrayT _ _) = T ∧
-  is_ArrayT _ = F
-End
-
-Definition lookup_function_def:
-  lookup_function name Deploy [] = SOME ([], NoneT, [Pass]) ∧
-  lookup_function name vis [] = NONE ∧
-  lookup_function name vis (FunctionDef fv fm id args ret body :: ts) =
-  (if id = name ∧ vis = fv then SOME (args, ret, body)
-   else lookup_function name vis ts) ∧
-  lookup_function name External (VariableDecl Public _ id typ :: ts) =
-  (if id = name ∧ ¬is_ArrayT typ then SOME ([], typ, [Return (SOME (TopLevelName id))])
-   else lookup_function name External ts) ∧
- (* TODO: handle arrays, array of array, hashmap of array, etc. *)
- (* TODO
-  lookup_function name External (HashMapDecl Public id kt vt :: ts) =
-  (if id = name then SOME ([("], typ, [Return (SOME (TopLevelName "id"))])
-   else lookup_function name External ts) ∧
- *)
-  lookup_function name vis (_ :: ts) =
-    lookup_function name vis ts
-End
-
-val () = cv_auto_trans lookup_function_def;
-
-Definition push_call_def:
-  push_call ct args ctx =
-  case ct of IntCall fn =>
-    if ctx.current_fc.name = Fn fn ∨
-       EXISTS (λfc. fc.name = Fn fn) ctx.call_stack
-    then raise (Error "recursive call") ctx else (
-    case lookup_function fn Internal ctx.current_contract.src of
-    | SOME (params, ret, body) =>
-      (case bind_arguments params args of
-       | SOME env =>
-           let fc = initial_function_context fn env body in
-           ctx with <|
-             call_stack updated_by CONS ctx.current_fc
-           ; current_fc := fc |>
-       | _ => raise (Error "bind_arguments") ctx)
-    | _ => raise (Error "lookup_function Internal") ctx )
-  (* TODO: support Send and ExtCall *)
-  | _ => raise (Error "unsupported call") ctx
-End
-
-val () = cv_auto_trans push_call_def;
-
-Definition update_current_stmt_def:
-  update_current_statement st ctx =
-  ctx with current_fc updated_by
-    (λfc. fc with current_stmt := st)
-End
-
-val () = cv_auto_trans update_current_stmt_def;
-
-Definition return_expr_def:
-  return_expr v (StartExpr _) = ErrorExpr "return StartExpr" ∧
-  return_expr v (IfExpK k e1 e2) = IfExpK (return_expr v k) e1 e2  ∧
-  return_expr v (ArrayLitK b vs k es) = ArrayLitK b vs (return_expr v k) es ∧
-  return_expr v (SubscriptK1 k e) = SubscriptK1 (return_expr v k) e ∧
-  return_expr v (SubscriptK2 w k) = SubscriptK2 w (return_expr v k) ∧
-  return_expr v (SubscriptMapK h k) = SubscriptMapK h (return_expr v k) ∧
-  return_expr v (AttributeK k id) = AttributeK (return_expr v k) id ∧
-  return_expr v (BuiltinK bt vs k es) = BuiltinK bt vs (return_expr v k) es ∧
-  return_expr v (CallK id vs k es) = CallK id vs (return_expr v k) es ∧
-  return_expr v (LiftCall fn vs k) = LiftCall fn vs (return_expr v k) ∧
-  return_expr v (DoneExpr _) = ErrorExpr "return DoneExpr" ∧
-  return_expr v (DoneExprMap _) = ErrorExpr "return DoneExprMap" ∧
-  return_expr v ReturnExpr = DoneExpr v ∧
-  return_expr v (ErrorExpr msg) = ErrorExpr msg
-End
-
-val () = cv_auto_trans return_expr_def;
-
-Definition return_base_tgt_def:
-  return_base_tgt v (StartBaseTgt _) = ErrorBaseTgt "return_base_tgt Start" ∧
-  return_base_tgt v (SubscriptTargetK1 k e) =
-    SubscriptTargetK1 (return_base_tgt v k) e ∧
-  return_base_tgt v (SubscriptTargetK2 l s k) =
-    SubscriptTargetK2 l s (return_expr v k) ∧
-  return_base_tgt v (AttributeTargetK k id) =
-    AttributeTargetK (return_base_tgt v k) id ∧
-  return_base_tgt v (LiftCallBaseTgt fn vs k) =
-    LiftCallBaseTgt fn vs (return_base_tgt v k) ∧
-  return_base_tgt _ (DoneBaseTgt _ _) = ErrorBaseTgt "return_base_tgt Done" ∧
-  return_base_tgt _ (ErrorBaseTgt msg) = ErrorBaseTgt msg
-End
-
-val () = cv_auto_trans return_base_tgt_def;
-
-Definition return_tgt_def:
-  return_tgt v (StartTgt _) = ErrorTgt "return StartTgt" ∧
-  return_tgt v (TupleTargetK vs k as) =
-    TupleTargetK vs (return_tgt v k) as ∧
-  return_tgt v (BaseTargetK t) =
-    (case return_base_tgt v t of ErrorBaseTgt msg => ErrorTgt msg
-        | t => BaseTargetK t) ∧
-  return_tgt v (LiftCallTgt fn vs k) =
-    LiftCallTgt fn vs (return_tgt v k) ∧
-  return_tgt v (DoneTgt _) = ErrorTgt "return DoneTgt" ∧
-  return_tgt v (ErrorTgt msg) = ErrorTgt msg
-End
-
-val () = cv_auto_trans return_tgt_def;
-
-Definition return_def:
-  return v (ForK id typ k n ss) = ForK id typ (return_expr v k) n ss ∧
-  return v (IfK k s1 s2) = IfK (return_expr v k) s1 s2 ∧
-  return v (AssertK k s) = AssertK (return_expr v k) s ∧
-  return v (ReturnSomeK k) = ReturnSomeK (return_expr v k) ∧
-  return v (AssignK1 t e) = AssignK1 (return_tgt v t) e ∧
-  return v (AssignK2 a k) = AssignK2 a (return_expr v k) ∧
-  return v (AugAssignK1 bt op e) = AugAssignK1 (return_base_tgt v bt) op e ∧
-  return v (AugAssignK2 l sl op k) = AugAssignK2 l sl op (return_expr v k) ∧
-  return v (AnnAssignK id typ k) = AnnAssignK id typ (return_expr v k) ∧
-  return v (StartK _) = ExceptionK (Error "return StartK") ∧
-  return v (ExprK k) = ExprK (return_expr v k) ∧
-  return v (DoneK) = ExceptionK (Error "return DoneK") ∧
-  return v (ExceptionK err) = ExceptionK (Error "return ExceptionK")
-End
-
-val () = cv_auto_trans return_def;
-
-Definition pop_call_def:
-  pop_call v ctx =
-  case ctx.call_stack of fc::fcs =>
-    if case fc.name of Loop _ => T | _ => F then
-      pop_call v (ctx with call_stack := fcs)
-    else
-      ctx with <|
-          current_fc := fc with current_stmt updated_by return v
-        ; call_stack := fcs
-        |>
-  | _ => raise (ExternalReturn v) ctx
+Definition eval_expr_cps_def:
+  eval_expr_cps cx1 (Name id) st k =
+    liftk cx1 ApplyTv
+      (do env <- get_scopes;
+          v <- lift_option (lookup_scopes (string_to_num id) env) "lookup Name";
+          return $ Value v od st) k ∧
+  eval_expr_cps cx2 (TopLevelName id) st k =
+    liftk cx2 ApplyTv (lookup_global cx2 (string_to_num id) st) k ∧
+  eval_expr_cps cx3 (IfExp e1 e2 e3) st k =
+    eval_expr_cps cx3 e1 st (IfExpK e2 e3 k) ∧
+  eval_expr_cps cx4 (Literal l) st k =
+    AK cx4 (ApplyTv (Value $ evaluate_literal l)) st k ∧
+  eval_expr_cps cx5 (ArrayLit b es) st k =
+    (case check (compatible_bound b (LENGTH es)) "ArrayLit bound" st of
+       (INR ex, st) => AK cx5 (ApplyExc ex) st k
+     | (INL (), st) => eval_exprs_cps cx5 es st (ArrayLitK b k)) ∧
+  eval_expr_cps cx6 (Subscript e1 e2) st k =
+    eval_expr_cps cx6 e1 st (SubscriptK e2 k) ∧
+  eval_expr_cps cx7 (Attribute e id) st k =
+    eval_expr_cps cx7 e st (AttributeK id k) ∧
+  eval_expr_cps cx8 (Builtin bt es) st k =
+    (case check (builtin_args_length_ok bt (LENGTH es)) "Builtin args" st of
+       (INR ex, st) => AK cx8 (ApplyExc ex) st k
+     | (INL (), st) => eval_exprs_cps cx8 es st (BuiltinK bt k)) ∧
+  eval_expr_cps cx9 (Call Send es) st k =
+    (case check (LENGTH es = 2) "Send args" st of
+       (INR ex, st) => AK cx9 (ApplyExc ex) st k
+     | (INL (), st) => eval_exprs_cps cx9 es st (CallSendK k)) ∧
+  eval_expr_cps cx10 (Call (ExtCall _) _) st k =
+    AK cx10 (ApplyExc (Error "TODO: ExtCall")) st k ∧
+  eval_expr_cps cx10 (Call (IntCall fn) es) st k =
+    (case do
+      check (no_recursion fn cx10.stk) "recursion";
+      ts <- lift_option (get_self_code cx10) "IntCall get_self_code";
+      tup <- lift_option (lookup_function fn Internal ts) "IntCall lookup_function";
+      args <<- FST tup; body <<- SND $ SND tup;
+      check (LENGTH args = LENGTH es) "IntCall args length";
+      return (args, body) od st
+     of (INR ex, st) => AK cx10 (ApplyExc ex) st k
+      | (INL (args, body), st) =>
+          eval_exprs_cps cx10 es st (IntCallK fn args body k)) ∧
+  eval_exprs_cps cx11 [] st k = AK cx11 (ApplyVals []) st k ∧
+  eval_exprs_cps cx12 (e::es) st k =
+    eval_expr_cps cx12 e st (ExprsK es k)
 Termination
-  WF_REL_TAC`measure (λx. LENGTH (SND x).call_stack)` \\ rw[]
+  WF_REL_TAC ‘measure (λx. case x of
+    | INL (cx,e,st,k) => expr_size e
+    | INR (cx,es,st,k) => list_size expr_size es)’
 End
 
-val pop_call_pre_def = cv_auto_trans_pre pop_call_def;
+val option_CASE_rator =
+  DatatypeSimps.mk_case_rator_thm_tyinfo
+    (Option.valOf (TypeBase.read {Thy="option",Tyop="option"}));
 
-Theorem pop_call_pre[cv_pre]:
-  ∀v ctx. pop_call_pre v ctx
+val sum_CASE_rator =
+  DatatypeSimps.mk_case_rator_thm_tyinfo
+    (Option.valOf (TypeBase.read {Thy="sum",Tyop="sum"}));
+
+val prod_CASE_rator =
+  DatatypeSimps.mk_case_rator_thm_tyinfo
+    (Option.valOf (TypeBase.read {Thy="pair",Tyop="prod"}));
+
+val toplevel_value_CASE_rator =
+  DatatypeSimps.mk_case_rator_thm_tyinfo
+    (Option.valOf (TypeBase.read {Thy="vyperInterpreter",Tyop="toplevel_value"}));
+
+val eval_expr_cps_pre_def = eval_expr_cps_def
+   |> SRULE
+        [liftk1, bind_def, ignore_bind_def,
+         LET_RATOR, option_CASE_rator,
+         sum_CASE_rator, prod_CASE_rator, lift_option_def]
+   |> cv_auto_trans_pre;
+
+Theorem eval_expr_cps_pre[cv_pre]:
+  (∀a b c d. eval_expr_cps_pre a b c d) ∧
+  (∀x y z w. eval_exprs_cps_pre x y z w)
 Proof
-  ho_match_mp_tac pop_call_ind
-  \\ rw[]
-  \\ rw[Once pop_call_pre_def]
-  \\ fs[]
-  \\ qmatch_assum_abbrev_tac`pop_call_pre v c1`
-  \\ qmatch_goalsub_abbrev_tac`pop_call_pre v c2`
-  \\ `c1 = c2` suffices_by (rw[] \\ fs[])
-  \\ rw[Abbr`c1`, Abbr`c2`]
-  \\ CASE_TAC
-  \\ rw[ theorem"execution_context_component_equality"]
+  ho_match_mp_tac eval_expr_cps_ind \\ rw[]
+  \\ rw[Once eval_expr_cps_pre_def]
+  \\ gvs[CaseEq"prod", CaseEq"sum", CaseEq"option", raise_def, check_def]
+  \\ first_x_assum irule
+  \\ gvs[bind_def, ignore_bind_def, lift_option_def]
 QED
 
-Definition set_stmt_def:
-  set_stmt k ctx =
-    ctx with current_fc updated_by (λfc. fc with current_stmt := k)
+Definition eval_base_target_cps_def:
+  eval_base_target_cps cx (NameTarget id) st k =
+    (let r = do
+        sc <- get_scopes;
+        n <<- string_to_num id;
+        cs <- lift_option (find_containing_scope n sc) "NameTarget lookup";
+        return $ (ScopedVar cs id, []) od st in
+     liftk cx ApplyBaseTarget r k) ∧
+  eval_base_target_cps cx (TopLevelNameTarget id) st k =
+    AK cx (ApplyBaseTarget (TopLevelVar id, [])) st k ∧
+  eval_base_target_cps cx (AttributeTarget t id) st k =
+    eval_base_target_cps cx t st (AttributeTargetK id k) ∧
+  eval_base_target_cps cx (SubscriptTarget t e) st k =
+    eval_base_target_cps cx t st (SubscriptTargetK e k)
 End
 
-val () = cv_auto_trans set_stmt_def;
+val () = eval_base_target_cps_def
+  |> SRULE [bind_def, ignore_bind_def,
+            LET_RATOR, lift_option_def,
+            prod_CASE_rator, sum_CASE_rator,
+            option_CASE_rator, liftk1]
+  |> cv_auto_trans;
 
-Definition exception_raised_def:
-  exception_raised ctx <=>
-  case ctx.current_fc.current_stmt of ExceptionK _ => T | _ => F
+Definition eval_target_cps_def:
+  eval_target_cps cx (BaseTarget t) st k =
+    eval_base_target_cps cx t st (BaseTargetK k) ∧
+  eval_target_cps cx (TupleTarget gs) st k =
+    eval_targets_cps cx gs st (TupleTargetK k) ∧
+  eval_targets_cps cx [] st k = AK cx (ApplyTargets []) st k ∧
+  eval_targets_cps cx (g::gs) st k =
+    eval_target_cps cx g st (TargetsK gs k)
 End
 
-val () = cv_auto_trans exception_raised_def;
+val () = eval_target_cps_def |> cv_auto_trans;
 
-Definition push_loop_def:
-  push_loop id typ (v::vs) (s::ss) ctx =
-    ctx with <|
-      call_stack updated_by CONS ctx.current_fc
-    ; current_fc := <|
-        scopes := (FEMPTY |+ (id,v))::ctx.current_fc.scopes
-      ; current_stmt := (StartK s)
-      ; remaining_stmts := ss
-      ; name := Loop <|
-          loop_var := id
-        ; remaining_values := vs
-        ; loop_first_stmt := s
-        ; loop_rest_stmts := ss
-        |>
-      |>
-    |> ∧
-  push_loop _ _ [] (_::_) ctx = set_stmt DoneK ctx ∧
-  push_loop _ _ _ _ ctx = raise (Error "push_loop") ctx
+Definition eval_stmt_cps_def:
+  eval_stmt_cps cx Pass st k = AK cx Apply st k ∧
+  eval_stmt_cps cx Continue st k = AK cx (ApplyExc ContinueException) st k ∧
+  eval_stmt_cps cx Break st k = AK cx (ApplyExc BreakException) st k ∧
+  eval_stmt_cps cx (Return NONE) st k = AK cx (ApplyExc (ReturnException NoneV)) st k ∧
+  eval_stmt_cps cx (Return (SOME e)) st k = eval_expr_cps cx e st (ReturnK k) ∧
+  eval_stmt_cps cx (Raise str) st k = AK cx (ApplyExc (AssertException str)) st k ∧
+  eval_stmt_cps cx (Assert e str) st k = eval_expr_cps cx e st (AssertK str k) ∧
+  eval_stmt_cps cx (AnnAssign id typ e) st k =
+    eval_expr_cps cx e st (AnnAssignK id k) ∧
+  eval_stmt_cps cx (Assign g e) st k =
+    eval_target_cps cx g st (AssignK e k) ∧
+  eval_stmt_cps cx (AugAssign t bop e) st k =
+    eval_base_target_cps cx t st (AugAssignK bop e k) ∧
+  eval_stmt_cps cx (If e ss1 ss2) st k =
+    eval_expr_cps cx e st (IfK ss1 ss2 k) ∧
+  eval_stmt_cps cx (For id typ e n body) st k =
+    eval_expr_cps cx e st (ForK id n body k) ∧
+  eval_stmt_cps cx (Expr e) st k =
+    eval_expr_cps cx e st (ExprK k)
 End
 
-val () = cv_auto_trans push_loop_def;
+val () = cv_auto_trans eval_stmt_cps_def;
 
-Definition pop_loop_def:
-  pop_loop ctx =
-  case ctx.call_stack of
-     | [] => raise (Error "pop_loop") ctx
-     | fc::fcs => ctx with <|
-         current_fc := (fc with <|
-           current_stmt := DoneK (* check it was ForK? *)
-         ; scopes := ctx.current_fc.scopes
-             (* TODO: is this a reason to maybe not have a loop context?  *)
-         |>)
-       ; call_stack := fcs |>
+Definition eval_stmts_cps_def:
+  eval_stmts_cps cx [] st k = AK cx Apply st k ∧
+  eval_stmts_cps cx (s::ss) st k =
+    eval_stmt_cps cx s st (StmtsK ss k)
 End
 
-val () = cv_auto_trans pop_loop_def;
+val () = cv_auto_trans eval_stmts_cps_def;
 
-Definition next_iteration_def:
-  next_iteration lp ctx =
-  case lp.remaining_values of [] => pop_loop ctx
-     | v::vs => ctx with current_fc updated_by (λfc.
-        fc with <| scopes updated_by CONS (FEMPTY |+ (lp.loop_var, v))
-                 ; current_stmt := StartK lp.loop_first_stmt
-                 ; remaining_stmts := lp.loop_rest_stmts
-                 ; name := Loop (lp with remaining_values := vs) |>)
+Definition eval_for_cps_def:
+  eval_for_cps cx nm body [] st k = AK cx Apply st k ∧
+  eval_for_cps cx nm body (v::vs) st k =
+  (case push_scope_with_var nm v st of
+        (INR ex, st) => AK cx (ApplyExc ex) st k
+      | (INL (), st) => eval_stmts_cps cx body st (ForK1 nm body vs k))
 End
 
-val () = cv_auto_trans next_iteration_def;
+val () = cv_auto_trans eval_for_cps_def;
 
-Definition continue_loop_def:
-  continue_loop ctx =
-  case ctx.current_fc.name of Loop lp => (
-    let ctx = pop_scope ctx in
-      if exception_raised ctx then ctx else
-        next_iteration lp ctx
-  ) | _ => raise (Error "continue_loop") ctx
+Definition apply_def:
+  apply cx st (StmtsK ss k) =
+    eval_stmts_cps cx ss st k ∧
+  apply cx st (ForK1 nm body vs k) =
+    (case pop_scope st
+     of (INR ex, st) => AK cx (ApplyExc ex) st k
+      | (INL (), st) => eval_for_cps cx nm body vs st k) ∧
+  apply cx st (IfK2 k) =
+    (case pop_scope st
+     of (INR ex, st) => AK cx (ApplyExc ex) st k
+      | (INL (), st) => AK cx Apply st k) ∧
+  apply cx st (IfK1 (Value (BoolV b)) ss1 ss2 k) =
+    eval_stmts_cps cx (if b then ss1 else ss2) st (IfK2 k) ∧
+  apply cx st (IfK1 (Value _) ss1 ss2 k) =
+    AK cx (ApplyExc $ Error "not BoolV") st (IfK2 k) ∧
+  apply cx st (IfK1 _ ss1 ss2 k) =
+    AK cx (ApplyExc $ Error "not Value") st (IfK2 k) ∧
+  apply cx st (IntCallK1 prev k) =
+    liftk (cx with stk updated_by TL) (ApplyTv o Value)
+      (do pop_function prev; return NoneV od st) k ∧
+  apply cx st DoneK = AK cx Apply st DoneK ∧
+  apply cx st _ = AK cx (ApplyExc $ Error "apply k") st DoneK
 End
 
-val () = cv_auto_trans continue_loop_def;
+val () = apply_def
+  |> SRULE [liftk1, ignore_bind_def, bind_def, prod_CASE_rator, sum_CASE_rator]
+  |> cv_auto_trans;
 
-Definition break_loop_def:
-  break_loop ctx =
-  case ctx.current_fc.name of Loop lp => (
-    let ctx = pop_scope ctx in
-      if exception_raised ctx then ctx else
-        pop_loop ctx
-  ) | _ => raise (Error "break_loop") ctx
+Definition apply_exc_def:
+  apply_exc cx ex st (ReturnK k) = AK cx (ApplyExc ex) st k ∧
+  apply_exc cx ex st (AssertK _ k) = AK cx (ApplyExc ex) st k ∧
+  apply_exc cx ex st (AnnAssignK _ k) = AK cx (ApplyExc ex) st k ∧
+  apply_exc cx ex st (AssignK _ k) = AK cx (ApplyExc ex) st k ∧
+  apply_exc cx ex st (AssignK1 _ k) = AK cx (ApplyExc ex) st k ∧
+  apply_exc cx ex st (AugAssignK _ _ k) = AK cx (ApplyExc ex) st k ∧
+  apply_exc cx ex st (AugAssignK1 _ _ k) = AK cx (ApplyExc ex) st k ∧
+  apply_exc cx ex st (IfK _ _ k) = AK cx (ApplyExc ex) st k ∧
+  apply_exc cx ex st (IfK1 _ _ _ k) = AK cx (ApplyExc ex) st k ∧
+  apply_exc cx ex st (IfK2 k) =
+    (case pop_scope st
+     of (INR ex, st) => AK cx (ApplyExc ex) st k
+      | (INL (), st) => AK cx (ApplyExc ex) st k) ∧
+  apply_exc cx ex st (ForK _ _ _ k) = AK cx (ApplyExc ex) st k ∧
+  apply_exc cx ex st (ForK1 nm body vs k) =
+    (case finally (handle_loop_exception ex) pop_scope st
+     of (INR ex, st) => AK cx (ApplyExc ex) st k
+      | (INL broke, st) =>
+          if broke then AK cx Apply st k
+          else eval_for_cps cx nm body vs st k) ∧
+  apply_exc cx ex st (ExprK k) = AK cx (ApplyExc ex) st k ∧
+  apply_exc cx ex st (StmtsK _ k) = AK cx (ApplyExc ex) st k ∧
+  apply_exc cx ex st (BaseTargetK k) = AK cx (ApplyExc ex) st k ∧
+  apply_exc cx ex st (TupleTargetK k) = AK cx (ApplyExc ex) st k ∧
+  apply_exc cx ex st (TargetsK _ k) = AK cx (ApplyExc ex) st k ∧
+  apply_exc cx ex st (TargetsK1 _ k) = AK cx (ApplyExc ex) st k ∧
+  apply_exc cx ex st (AttributeTargetK _ k) = AK cx (ApplyExc ex) st k ∧
+  apply_exc cx ex st (SubscriptTargetK _ k) = AK cx (ApplyExc ex) st k ∧
+  apply_exc cx ex st (SubscriptTargetK1 _ k) = AK cx (ApplyExc ex) st k ∧
+  apply_exc cx ex st (IfExpK _ _ k) = AK cx (ApplyExc ex) st k ∧
+  apply_exc cx ex st (ArrayLitK _ k) = AK cx (ApplyExc ex) st k ∧
+  apply_exc cx ex st (SubscriptK _ k) = AK cx (ApplyExc ex) st k ∧
+  apply_exc cx ex st (SubscriptK1 _ k) = AK cx (ApplyExc ex) st k ∧
+  apply_exc cx ex st (AttributeK _ k) = AK cx (ApplyExc ex) st k ∧
+  apply_exc cx ex st (BuiltinK _ k) = AK cx (ApplyExc ex) st k ∧
+  apply_exc cx ex st (CallSendK k) = AK cx (ApplyExc ex) st k ∧
+  apply_exc cx ex st (IntCallK _ _ _ k) = AK cx (ApplyExc ex) st k ∧
+  apply_exc cx ex st (IntCallK1 prev k) =
+    liftk (cx with stk updated_by TL) (ApplyTv o Value)
+      (finally (handle_function ex) (pop_function prev) st)
+      k ∧
+  apply_exc cx ex st (ExprsK _ k) = AK cx (ApplyExc ex) st k ∧
+  apply_exc cx ex st (ExprsK1 _ k) = AK cx (ApplyExc ex) st k ∧
+  apply_exc cx ex st DoneK = AK cx (ApplyExc ex) st DoneK
 End
 
-val () = cv_auto_trans break_loop_def;
+val () = apply_exc_def
+  |> SRULE [finally_def, bind_def, ignore_bind_def,
+            liftk1, prod_CASE_rator, sum_CASE_rator]
+  |> cv_auto_trans;
 
-Definition next_stmt_def:
-  next_stmt ctx =
-  case ctx.current_fc.remaining_stmts of s::ss =>
-    ctx with current_fc updated_by (λfc.
-      fc with <| current_stmt := StartK s
-               ; remaining_stmts := ss |>)
-  | _ => (case ctx.current_fc.name
-            of Fn _ => pop_call NoneV ctx
-             | Loop lp =>
-                 let ctx = pop_scope ctx in
-                   if exception_raised ctx then ctx
-                   else next_iteration lp ctx)
+Definition apply_targets_def:
+  apply_targets cx gvs st (TargetsK1 gv k) =
+    AK cx (ApplyTargets (gv::gvs)) st k ∧
+  apply_targets cx gvs st (TupleTargetK k) =
+      AK cx (ApplyTarget (TupleTargetV gvs)) st k ∧
+  apply_targets cx _ st _ =
+    AK cx (ApplyExc $ Error "apply_targets k") st DoneK
 End
 
-val () = cv_auto_trans next_stmt_def;
+val () = cv_auto_trans apply_targets_def;
 
-Definition step_stmt_start_def:
-  step_stmt_start Pass ctx = set_stmt DoneK ctx ∧
-  step_stmt_start Continue ctx = continue_loop ctx ∧
-  step_stmt_start Break ctx = break_loop ctx ∧
-  step_stmt_start (Expr e) ctx = set_stmt (ExprK (StartExpr e)) ctx ∧
-  step_stmt_start (Raise s) ctx = raise (RaiseException s) ctx ∧
-  step_stmt_start (Assert e s) ctx = set_stmt (AssertK (StartExpr e) s) ctx ∧
-  step_stmt_start (Return NONE) ctx = pop_call NoneV ctx ∧
-  step_stmt_start (Return (SOME e)) ctx =
-    set_stmt (ReturnSomeK (StartExpr e)) ctx ∧
-  step_stmt_start (AnnAssign id typ e) ctx =
-    set_stmt (AnnAssignK id typ (StartExpr e)) ctx ∧
-  step_stmt_start (AugAssign bt bop e) ctx =
-    set_stmt (AugAssignK1 (StartBaseTgt bt) bop e) ctx ∧
-  step_stmt_start (Assign tgt e) ctx =
-    set_stmt (AssignK1 (StartTgt tgt) e) ctx ∧
-  step_stmt_start (If e s1 s2) ctx =
-    set_stmt (IfK (StartExpr e) s1 s2) ctx ∧
-  step_stmt_start (For id typ e n s) ctx =
-    set_stmt (ForK id typ (StartExpr e) n s) ctx
+Definition apply_base_target_def:
+  apply_base_target cx btv st (BaseTargetK k) =
+    AK cx (ApplyTarget (BaseTargetV (FST btv) (SND btv))) st k ∧
+  apply_base_target cx btv st (AttributeTargetK id k) =
+    AK cx (ApplyBaseTarget (FST btv, AttrSubscript id :: SND btv)) st k ∧
+  apply_base_target cx btv st (SubscriptTargetK e k) =
+    eval_expr_cps cx e st (SubscriptTargetK1 btv k) ∧
+  apply_base_target cx btv st (AugAssignK bop e k) =
+    eval_expr_cps cx e st (AugAssignK1 btv bop k) ∧
+  apply_base_target cx btv st DoneK = AK cx (ApplyBaseTarget btv) st DoneK ∧
+  apply_base_target cx _ st _ =
+    AK cx (ApplyExc $ Error "apply_base_target k") st DoneK
 End
 
-val () = cv_auto_trans step_stmt_start_def;
+val () = cv_auto_trans apply_base_target_def;
 
-Datatype:
-  step_stmt_expr_result
-  = RVal value
-  | RErr string
-  | RCall call_target (value list) expr_continuation
-  | RElse expr_continuation
+Definition apply_target_def:
+  apply_target cx gv st (AssignK e k) =
+    eval_expr_cps cx e st (AssignK1 gv k) ∧
+  apply_target cx gv st (TargetsK gs k) =
+    eval_targets_cps cx gs st (TargetsK1 gv k) ∧
+  apply_target cx gv st _ =
+    AK cx (ApplyExc $ Error "apply_target k") st DoneK
 End
 
-Definition step_stmt_expr_case_def:
-  step_stmt_expr_case (DoneExpr v) = RVal v ∧
-  step_stmt_expr_case (DoneExprMap _) = RErr "Map" ∧
-  step_stmt_expr_case (ErrorExpr msg) = RErr msg ∧
-  step_stmt_expr_case (LiftCall fn vs k) = RCall fn vs k ∧
-  step_stmt_expr_case k = RElse k
+val () = cv_auto_trans apply_target_def;
+
+Definition apply_tv_def:
+  apply_tv cx tv st (SubscriptK e k) =
+    eval_expr_cps cx e st (SubscriptK1 tv k) ∧
+  apply_tv cx tv st (IfK ss1 ss2 k) =
+    liftk cx (K Apply) (push_scope st) (IfK1 tv ss1 ss2 k) ∧
+  apply_tv cx tv st DoneK = AK cx (ApplyTv tv) st DoneK ∧
+  apply_tv cx tv st k =
+    liftk cx ApplyVal (get_Value tv st) k
 End
 
-val () = cv_auto_trans step_stmt_expr_case_def;
+val () = apply_tv_def
+  |> SRULE [liftk1, prod_CASE_rator, sum_CASE_rator]
+  |> cv_auto_trans;
 
-Definition step_stmt_def:
-  step_stmt ctx =
-  let fc = ctx.current_fc in
-  let gbs = ctx.current_contract.globals in
-  let tx = ctx.current_transaction in
-  let ectx =
-    <| tx := tx; gbs := gbs; env := fc.scopes;
-       bal := ctx.current_balances |> in
-  (case fc.current_stmt of
-      | StartK st => step_stmt_start st ctx
-      | ExprK k => (case step_stmt_expr_case k of
-          RVal _ => set_stmt DoneK ctx
-        | RErr msg => raise (Error ("ExprK " ++ msg)) ctx
-        | RCall fn vs k => push_call fn vs (set_stmt (ExprK k) ctx)
-        | RElse k => set_stmt (ExprK (step_expr ectx k)) ctx)
-      | IfK k s1 s2 => (case step_stmt_expr_case k of
-          RVal (BoolV b) => (
-            case (if b then s1 else s2) of s::ss =>
-              ctx with current_fc := fc with
-                <| current_stmt := StartK s
-                 ; remaining_stmts updated_by (λx. ss ++ x) |>
-            | _ => set_stmt DoneK ctx)
-        | RVal _ => raise (Error "IfK not BoolV") ctx
-        | RErr msg => raise (Error ("IfK " ++ msg)) ctx
-        | RCall fn vs k => push_call fn vs (set_stmt (IfK k s1 s2) ctx)
-        | RElse k => set_stmt (IfK (step_expr ectx k) s1 s2) ctx)
-      | AssertK k s => (case step_stmt_expr_case k of
-          RVal (BoolV b) => (
-            if b then set_stmt DoneK ctx
-            else raise (AssertException s) ctx)
-        | RVal _ => raise (Error "AssertK not BoolV") ctx
-        | RErr msg => raise (Error ("AssertK " ++ msg)) ctx
-        | RCall fn vs k => push_call fn vs (set_stmt (AssertK k s) ctx)
-        | RElse k => set_stmt (AssertK (step_expr ectx k) s) ctx)
-      | ReturnSomeK k => (case step_stmt_expr_case k of
-          RVal v => pop_call v ctx
-        | RErr msg => raise (Error ("ReturnSomeK " ++ msg)) ctx
-        | RCall fn vs k => push_call fn vs (set_stmt (ReturnSomeK k) ctx)
-        | RElse k => set_stmt (ReturnSomeK (step_expr ectx k)) ctx)
-      | AssignK1 (DoneTgt av) e =>
-          set_stmt (AssignK2 av (StartExpr e)) ctx
-      | AssignK1 (ErrorTgt msg) e => raise (Error "AssignK1 err") ctx
-      | AssignK1 (LiftCallTgt fn vs tk) e =>
-          push_call fn vs
-            (set_stmt (AssignK1 tk e) ctx)
-      | AssignK1 tk e =>
-          set_stmt
-            (AssignK1 (step_target ectx tk) e) ctx
-      | AssignK2 tv k => (case step_stmt_expr_case k of
-          RVal v =>
-          let ctx = assign_target tv (Replace v) ctx in
-            if exception_raised ctx then ctx else
-              set_stmt DoneK ctx
-        | RErr msg => raise (Error ("AssignK2 " ++ msg)) ctx
-        | RCall fn vs k => push_call fn vs (set_stmt (AssignK2 tv k) ctx)
-        | RElse k => set_stmt (AssignK2 tv (step_expr ectx k)) ctx)
-      | AugAssignK1 (DoneBaseTgt l sl) bop e =>
-          set_stmt (AugAssignK2 l sl bop (StartExpr e)) ctx
-      | AugAssignK1 (LiftCallBaseTgt fn vs bk) bop e =>
-          push_call fn vs (set_stmt (AugAssignK1 bk bop e) ctx)
-      | AugAssignK1 bk bop e =>
-          set_stmt
-            (AugAssignK1 (step_base_target ectx bk) bop e) ctx
-      | AugAssignK2 l sl bop k => (case step_stmt_expr_case k of
-          RVal v2 =>
-          let ctx = assign_target (BaseTargetV l sl) (Update bop v2) ctx in
-            if exception_raised ctx then ctx else set_stmt DoneK ctx
-        | RErr msg => raise (Error ("AugAssignK2 " ++ msg)) ctx
-        | RCall fn vs k => push_call fn vs (set_stmt (AugAssignK2 l sl bop k) ctx)
-        | RElse k => set_stmt (AugAssignK2 l sl bop (step_expr ectx k)) ctx)
-      | AnnAssignK id typ k => (case step_stmt_expr_case k of
-          RVal v =>
-          let nid = string_to_num id in
-          let ctx = new_variable nid typ ctx in
-            if exception_raised ctx then ctx else
-              set_stmt DoneK (set_variable nid v ctx)
-        | RErr msg => raise (Error ("AnnAssignK " ++ msg)) ctx
-        | RCall fn vs k => push_call fn vs (set_stmt (AnnAssignK id typ k) ctx)
-        | RElse k => set_stmt (AnnAssignK id typ (step_expr ectx k)) ctx)
-      | ExceptionK err => ctx
-      | DoneK => next_stmt ctx
-      | ForK id typ (DoneExpr (ArrayV _ [])) n (st::ss) =>
-          set_stmt DoneK ctx
-      | ForK id typ (DoneExpr (ArrayV _ vs)) n ss =>
-          if LENGTH vs ≤ n then
-            push_loop (string_to_num id) typ vs ss ctx
-          else raise (Error "ForK bound") ctx
-      | ForK id typ (DoneExpr _) _ _ => raise (Error "ForK DoneExpr") ctx
-      | ForK id typ (DoneExprMap _) _ _ => raise (Error "ForK DoneExprMap") ctx
-      | ForK id typ (ErrorExpr msg) _ _ => raise (Error "ForK err") ctx
-      | ForK id typ ReturnExpr _ _ => raise (Error "ForK ReturnExpr") ctx
-      | ForK id typ (LiftCall fn vs k) n ss =>
-          push_call fn vs
-            (set_stmt (ForK id typ k n ss) ctx)
-      | ForK id typ k n ss =>
-          set_stmt (ForK id typ (step_expr ectx k) n ss) ctx)
+Definition apply_val_def:
+  apply_val cx v st (ReturnK k) = apply_exc cx (ReturnException v) st k ∧
+  apply_val cx (BoolV T) st (AssertK str k) = apply cx st k ∧
+  apply_val cx (BoolV F) st (AssertK str k) =
+    apply_exc cx (AssertException str) st k ∧
+  apply_val cx v st (AssertK _ k) = apply_exc cx (Error "not BoolV") st k ∧
+  apply_val cx v st (AnnAssignK id k) =
+    liftk cx (K Apply) (new_variable id v st) k ∧
+  apply_val cx v st (AssignK1 gv k) =
+    liftk cx (K Apply) (assign_target cx gv (Replace v) st) k ∧
+  apply_val cx v st (AugAssignK1 (loc, sbs) bop k) =
+    liftk cx (K Apply) (assign_target cx (BaseTargetV loc sbs) (Update bop v) st) k ∧
+  apply_val cx v st (ForK id n body k) =
+    (case do vs <- lift_option (extract_elements v) "For not ArrayV";
+             check (compatible_bound (Dynamic n) (LENGTH vs)) "For too long";
+             return vs od st
+     of (INR ex, st) => apply_exc cx ex st k
+      | (INL vs, st) => eval_for_cps cx (string_to_num id) body vs st k) ∧
+  apply_val cx v st (ExprK k) = apply cx st k ∧
+  apply_val cx v st (SubscriptTargetK1 (loc, sbs) k) =
+    (case lift_option (value_to_key v) "SubscriptTarget value_to_key" st
+       of (INR ex, st) => apply_exc cx ex st k
+        | (INL sk, st) => apply_base_target cx (loc, sk :: sbs) st k) ∧
+  apply_val cx (BoolV T) st (IfExpK e2 e3 k) =
+    eval_expr_cps cx e2 st k ∧
+  apply_val cx (BoolV F) st (IfExpK e2 e3 k) =
+    eval_expr_cps cx e3 st k ∧
+  apply_val cx v st (IfExpK _ _ k) =
+    apply_exc cx (Error "not BoolV") st k ∧
+  apply_val cx v2 st (SubscriptK1 tv1 k) =
+    liftk cx ApplyTv (lift_sum (evaluate_subscript tv1 v2) st) k ∧
+  apply_val cx v st (AttributeK id k) =
+    liftk cx (ApplyTv o Value) (lift_sum (evaluate_attribute v id) st) k ∧
+  apply_val cx v st (ExprsK es k) =
+    eval_exprs_cps cx es st (ExprsK1 v k) ∧
+  apply_val cx v st DoneK = AK cx (ApplyVal v) st DoneK ∧
+  apply_val cx v st _ =
+    AK cx (ApplyExc $ Error "apply_val k") st DoneK
 End
 
-val () = cv_auto_trans step_stmt_def;
+val () = apply_val_def
+  |> SRULE [liftk1, prod_CASE_rator, sum_CASE_rator,
+            option_CASE_rator, lift_option_def, lift_sum_def,
+            bind_def, ignore_bind_def]
+  |> cv_auto_trans;
 
-Definition expr_bound_def[simp]:
-  expr_bound (Name _, fns) = (0n, fns) ∧
-  expr_bound (TopLevelName _, fns) = (0, fns) ∧
-  expr_bound (IfExp e1 e2 e3, fns) = (
-    let (n1, fns) = expr_bound (e1, fns) in
-    let (n2, fns) = expr_bound (e2, fns) in
-    let (n3, fns) = expr_bound (e3, fns) in
-      (1 + n1 + MAX n2 n3, fns) ) ∧
-  expr_bound (Literal _, fns) = (0, fns) ∧
-  expr_bound (ArrayLit _ es, fns) = (
-  let (ns, fns) = expr_bound_list (es, fns) in
-    (1 + ns, fns) ) ∧
-  expr_bound (Subscript e1 e2, fns) = (
-  let (n1, fns) = expr_bound (e1, fns) in
-  let (n2, fns) = expr_bound (e2, fns) in
-    (1 + n1 + n2, fns) ) ∧
-  expr_bound (Attribute e _, fns) = (
-  let (n, fns) = expr_bound (e, fns) in
-    (1 + n, fns) ) ∧
-  expr_bound (Builtin _ es, fns) = (
-  let (ns, fns) = expr_bound_list (es, fns) in
-    (1 + ns, fns) ) ∧
-  expr_bound (Call ct es, fns) = (
-  let (ns, fns) = expr_bound_list (es, fns) in
-    (1 + ns, (case ct of IntCall fn => fn INSERT fns | _ => fns)) ) ∧
-  expr_bound_list ([], fns) = (0, fns) ∧
-  expr_bound_list (e::es, fns) = (
-  let (n, fns) = expr_bound (e, fns) in
-  let (ns, fns) = expr_bound_list (es, fns) in
-    (1 + n + ns, fns) )
-Termination
-  WF_REL_TAC`measure (λx.
-    case x of INL (e, _) => expr_size e
-            | INR (es, _) => expr1_size es)`
+Definition apply_vals_def:
+  apply_vals cx vs st (ExprsK1 v k) =
+    apply_vals cx (v::vs) st k ∧
+  apply_vals cx vs st (ArrayLitK b k) =
+    apply_tv cx (Value $ ArrayV b vs) st k ∧
+  apply_vals cx vs st (BuiltinK bt k) =
+    liftk cx ApplyTv (do
+      acc <- get_accounts;
+      v <- lift_sum $ evaluate_builtin cx acc bt vs;
+      return $ Value v
+    od st) k ∧
+  apply_vals cx vs st (CallSendK k) =
+    liftk cx ApplyTv (do
+      check (LENGTH vs = 2) "CallSendK nargs";
+      toAddr <- lift_option (dest_AddressV $ EL 0 vs) "Send not AddressV";
+      amount <- lift_option (dest_NumV $ EL 1 vs) "Send not NumV";
+      transfer_value cx.txn.sender toAddr amount;
+      return $ Value NoneV
+    od st) k ∧
+  apply_vals cx vs st (IntCallK fn args body k) =
+    (case do
+      env <- lift_option (bind_arguments args vs) "IntCall bind_arguments";
+      prev <- get_scopes;
+      cxf <- push_function fn env cx;
+      return (prev, cxf, body) od st
+     of (INR ex, st) => apply_exc cx ex st k
+      | (INL (prev, cxf, body), st) =>
+          eval_stmts_cps cxf body st (IntCallK1 prev k)) ∧
+  apply_vals cx vs st DoneK = AK cx (ApplyVals vs) st DoneK ∧
+  apply_vals cx vs st _ =
+    AK cx (ApplyExc $ Error "apply_vals k") st DoneK
 End
 
-Definition exprk_bound_def[simp]:
-  exprk_bound (StartExpr e, fns) = (
-    let (n, fns) = expr_bound (e, fns) in
-      (2 + n, fns)) ∧
-  exprk_bound (IfExpK k e1 e2, fns) = (
-    let (n, fns) = exprk_bound (k, fns) in
-    let (n1, fns) = expr_bound (e1, fns) in
-    let (n2, fns) = expr_bound (e2, fns) in
-      (1 + n + n2 + n2, fns)) ∧
-  exprk_bound (ArrayLitK _ _ k es, fns) = (
-    let (n, fns) = exprk_bound (k, fns) in
-    let (ns, fns) = expr_bound_list (es, fns) in
-      (1 + n + ns, fns)) ∧
-  exprk_bound (SubscriptK1 k e, fns) = (
-    let (n, fns) = exprk_bound (k, fns) in
-    let (ne, fns) = expr_bound (e, fns) in
-      (1 + n + ne, fns)) ∧
-  exprk_bound (SubscriptK2 _ k, fns) = (
-    let (n, fns) = exprk_bound (k, fns) in
-      (1 + n, fns)) ∧
-  exprk_bound (SubscriptMapK _ k, fns) = (
-    let (n, fns) = exprk_bound (k, fns) in
-      (1 + n, fns)) ∧
-  exprk_bound (AttributeK k _, fns) = (
-    let (n, fns) = exprk_bound (k, fns) in
-      (1 + n, fns)) ∧
-  exprk_bound (BuiltinK _ _ k es, fns) = (
-    let (n, fns) = exprk_bound (k, fns) in
-    let (ns, fns) = expr_bound_list (es, fns) in
-      (1 + n + ns, fns)) ∧
-  exprk_bound (CallK _ _ k es, fns) = (
-    let (n, fns) = exprk_bound (k, fns) in
-    let (ns, fns) = expr_bound_list (es, fns) in
-      (1 + n + ns, fns)) ∧
-  exprk_bound (LiftCall _ _ k, fns) = (
-    let (n, fns) = exprk_bound (k, fns) in
-      (1 + n, fns)) ∧
-  exprk_bound (DoneExpr _, fns) = (1, fns) ∧
-  exprk_bound (DoneExprMap _, fns) = (1, fns) ∧
-  exprk_bound (ReturnExpr, fns) = (1, fns) ∧
-  exprk_bound (ErrorExpr _, fns) = (1, fns)
-End
+val apply_vals_pre_def = apply_vals_def
+  |> SRULE [liftk1, bind_def, ignore_bind_def, lift_option_def,
+            lift_sum_def, prod_CASE_rator,
+            sum_CASE_rator, option_CASE_rator]
+  |> cv_auto_trans_pre;
 
-Definition base_tgt_bound_def[simp]:
-  base_tgt_bound (AttributeTarget t _, fns) =(
-  let (nt, fns) = base_tgt_bound (t, fns) in
-    (1 + nt, fns)) ∧
-  base_tgt_bound (SubscriptTarget t e, fns) = (
-  let (nt, fns) = base_tgt_bound (t, fns) in
-  let (ne, fns) = expr_bound (e, fns) in
-    (1 + nt + ne, fns)) ∧
-  base_tgt_bound (_, fns) = (1n, fns)
-End
-
-Definition tgt_bound_def[simp]:
-  tgt_bound (BaseTarget t, fns) = (
-  let (n, fns) = base_tgt_bound (t, fns) in
-    (1 + n, fns)) ∧
-  tgt_bound (TupleTarget ts, fns) = (
-  let (ns, fns) = tgt_bound_list (ts, fns) in
-    (1 + ns, fns)) ∧
-  tgt_bound_list ([], fns) = (0, fns) ∧
-  tgt_bound_list ((t::ts), fns) = (
-  let (n, fns) = tgt_bound (t, fns) in
-  let (ns, fns) = tgt_bound_list (ts, fns) in
-    (1 + n + ns, fns))
-Termination
-  WF_REL_TAC`measure (λx.
-    case x of INR (x, _) => assignment_target1_size x
-       | INL (x, _) => assignment_target_size x)`
-End
-
-Definition base_tgtk_bound_def[simp]:
-  base_tgtk_bound (StartBaseTgt t, fns) = (
-  let (n, fns) = base_tgt_bound (t, fns) in
-    (2 + n, fns)) ∧
-  base_tgtk_bound (SubscriptTargetK1 k e, fns) = (
-  let (n, fns) = base_tgtk_bound (k, fns) in
-  let (ne, fns) = expr_bound (e, fns) in
-    (1 + n + ne, fns)) ∧
-  base_tgtk_bound (SubscriptTargetK2 _ _ k, fns) = (
-  let (n, fns) = exprk_bound (k, fns) in
-    (1 + n, fns)) ∧
-  base_tgtk_bound (AttributeTargetK k _, fns) = (
-  let (n, fns) = base_tgtk_bound (k, fns) in
-    (1 + n, fns)) ∧
-  base_tgtk_bound (LiftCallBaseTgt _ _ k, fns) = (
-  let (n, fns) = base_tgtk_bound (k, fns) in
-    (1 + n, fns)) ∧
-  base_tgtk_bound (_, fns) = (1, fns)
-End
-
-Definition tgtk_bound_def[simp]:
-  tgtk_bound (StartTgt t, fns) = (
-  let (n, fns) = tgt_bound (t, fns) in
-    (2 + n, fns)) ∧
-  tgtk_bound (TupleTargetK _ k ts, fns) = (
-  let (n, fns) = tgtk_bound (k, fns) in
-  let (ns, fns) = tgt_bound_list (ts, fns) in
-    (1 + n + ns, fns)) ∧
-  tgtk_bound (BaseTargetK bk, fns) = (
-  let (n, fns) = base_tgtk_bound (bk, fns) in
-    (1 + n, fns)) ∧
-  tgtk_bound (LiftCallTgt _ _ k, fns) = (
-  let (n, fns) = tgtk_bound (k, fns) in
-    (1 + n, fns)) ∧
-  tgtk_bound (_, fns) = (1, fns)
-End
-
-Definition stmt_bound_def[simp]:
-  stmt_bound (Pass, fns) = (1n, fns) ∧
-  stmt_bound (Continue, fns) = (1, fns) ∧
-  stmt_bound (Break, fns) = (1, fns) ∧
-  stmt_bound (Expr e, fns) = (
-    let (ne, fns) = expr_bound (e, fns) in
-      (1 + ne, fns)) ∧
-  stmt_bound (For _ _ e n ss, fns) = (
-    let (ne, fns) = expr_bound (e, fns) in
-    let (ns, fns) = stmt_bound_list (ss, fns) in
-      (1 + ne + n * ns, fns)) ∧
-  stmt_bound (If e s1 s2, fns) = (
-    let (ne, fns) = expr_bound (e, fns) in
-    let (n1, fns) = stmt_bound_list (s1, fns) in
-    let (n2, fns) = stmt_bound_list (s2, fns) in
-      (1 + ne + n1 + n2, fns)) ∧
-  stmt_bound (Assert e _, fns) = (
-    let (ne, fns) = expr_bound (e, fns) in
-      (1 + ne, fns)) ∧
-  stmt_bound (Raise _, fns) = (1, fns) ∧
-  stmt_bound (Return NONE, fns) = (1, fns) ∧
-  stmt_bound (Return (SOME e), fns) = (
-    let (ne, fns) = expr_bound (e, fns) in
-      (1 + ne, fns)) ∧
-  stmt_bound (Assign tgt e, fns) = (
-    let (ne, fns) = expr_bound (e, fns) in
-    let (nt, fns) = tgt_bound (tgt, fns) in
-      (1 + ne + nt, fns)) ∧
-  stmt_bound (AugAssign bt _ e, fns) = (
-    let (ne, fns) = expr_bound (e, fns) in
-    let (nb, fns) = base_tgt_bound (bt, fns) in
-      (1 + ne + nb, fns)) ∧
-  stmt_bound (AnnAssign _ _ e, fns) = (
-    let (ne, fns) = expr_bound (e, fns) in
-      (1 + ne, fns)) ∧
-  stmt_bound_list ([], fns) = (0, fns) ∧
-  stmt_bound_list (s::ss, fns) = (
-    let (n, fns) = stmt_bound (s, fns) in
-    let (ns, fns) = stmt_bound_list (ss, fns) in
-      (1 + n + ns, fns))
-Termination
-  WF_REL_TAC`measure (λx.
-    case x of INL (e, _) => stmt_size e
-            | INR (es, _) => stmt1_size es)`
-End
-
-Definition stmtk_bound_def[simp]:
-  stmtk_bound (StartK s, fns) = (
-    let (n, fns) = stmt_bound (s, fns) in
-      (3 + n, fns)) ∧
-  stmtk_bound (ExprK k, fns) = (
-    let (n, fns) = exprk_bound (k, fns) in
-      (1 + n, fns)) ∧
-  stmtk_bound (IfK k s1 s2, fns) = (
-    let (n, fns) = exprk_bound (k, fns) in
-    let (n1, fns) = stmt_bound_list (s1, fns) in
-    let (n2, fns) = stmt_bound_list (s2, fns) in
-      (1 + n + n1 + n2, fns)) ∧
-  stmtk_bound (AssertK k _, fns) = (
-    let (n, fns) = exprk_bound (k, fns) in
-      (1 + n, fns)) ∧
-  stmtk_bound (ReturnSomeK k, fns) = (
-    let (n, fns) = exprk_bound (k, fns) in
-      (1 + n, fns)) ∧
-  stmtk_bound (AssignK1 tk e, fns) = (
-    let (nt, fns) = tgtk_bound (tk, fns) in
-    let (ne, fns) = expr_bound (e, fns) in
-      (1 + nt + ne, fns)) ∧
-  stmtk_bound (AssignK2 _ k, fns) = (
-    let (n, fns) = exprk_bound (k, fns) in
-      (1 + n, fns)) ∧
-  stmtk_bound (AugAssignK1 k _ e, fns) = (
-    let (n, fns) = base_tgtk_bound (k, fns) in
-    let (ne, fns) = expr_bound (e, fns) in
-      (1 + n + ne, fns)) ∧
-  stmtk_bound (AugAssignK2 _ _ _ k, fns) = (
-    let (n, fns) = exprk_bound (k, fns) in
-      (1 + n, fns)) ∧
-  stmtk_bound (AnnAssignK _ _ k, fns) = (
-    let (n, fns) = exprk_bound (k, fns) in
-      (1 + n, fns)) ∧
-  stmtk_bound (ForK _ _ k n s, fns) = (
-    let (nk, fns) = exprk_bound (k, fns) in
-    let (ns, fns) = stmt_bound_list (s, fns) in
-      (1 + nk + n * ns, fns)) ∧
-  stmtk_bound (_, fns) = (1, fns)
-End
-
-Definition fns_from_context_def:
-  fns_from_context fc =
-  case fc.name of Fn fn => {fn} | _ => {}
-End
-
-Definition all_fns_def[simp]:
-  all_fns [] = {} ∧
-  all_fns (FunctionDef fv fm id args ret body :: ts) =
-    id INSERT (all_fns ts) ∧
-  all_fns (_ :: ts) = all_fns ts
-End
-
-Definition fn_bound_def:
-  fn_bound ts all seen fns =
-  if FINITE all ∧ DISJOINT seen fns ∧ fns ⊆ all ∧ seen ⊆ all then
-    if fns = {} then 0 else
-      let fn = CHOICE fns in
-      let rest = REST fns in
-      let seen = fn INSERT seen in
-        case lookup_function fn Internal ts of
-           | NONE => fn_bound ts all seen rest
-           | SOME (_, _, body) =>
-             let (n, x) = stmt_bound_list (body, {}) in
-               n + fn_bound ts all seen (rest UNION (x DIFF seen))
-  else 0
-Termination
-  WF_REL_TAC`measure (λ(_,all,seen,_). CARD (all DIFF seen))`
-  \\ rw[]
-  \\ qmatch_goalsub_abbrev_tac`CARD s1 < CARD s2`
-  \\ `s2 = CHOICE fns INSERT s1`
-  by (
-    simp[Abbr`s1`, Abbr`s2`, EXTENSION]
-    \\ gs[IN_DISJOINT, SUBSET_DEF]
-    \\ rw[EQ_IMP_THM]
-    \\ metis_tac[CHOICE_DEF] )
-  \\ `FINITE s1` by rw[Abbr`s1`]
-  \\ rw[CARD_INSERT, Abbr`s1`]
-End
-
-Definition step_bound_def:
-  step_bound ctx =
-  let current_fns =
-    fns_from_context ctx.current_fc ∪
-    BIGUNION (IMAGE fns_from_context (set ctx.call_stack)) in
-  let ts = ctx.current_contract.src in
-  let (ns, fns) = stmtk_bound (ctx.current_fc.current_stmt, {}) in
-  let (nr, fns) = stmt_bound_list (ctx.current_fc.remaining_stmts, fns) in
-    ns + nr +
-      fn_bound ts (all_fns ts) current_fns (fns DIFF current_fns)
-End
-
-Theorem set_stmt_simps[simp]:
-  (set_stmt k ctx).current_contract = ctx.current_contract ∧
-  (set_stmt k ctx).call_stack = ctx.call_stack ∧
-  (set_stmt k ctx).current_fc.current_stmt = k ∧
-  (set_stmt k ctx).current_fc.remaining_stmts = ctx.current_fc.remaining_stmts
+Theorem apply_vals_pre[cv_pre]:
+  ∀a b c d. apply_vals_pre a b c d
 Proof
-  rw[set_stmt_def]
+  ho_match_mp_tac apply_vals_ind \\ rw[]
+  \\ rw[Once apply_vals_pre_def]
+  \\ gvs[check_def, assert_def]
+  \\ strip_tac \\ gvs[]
 QED
 
-Theorem fns_from_context_set_stmt[simp]:
-  fns_from_context (set_stmt k ctx).current_fc =
-  fns_from_context ctx.current_fc
-Proof
-  rw[set_stmt_def, fns_from_context_def]
-QED
+Definition nextk_def[simp]:
+  nextk (AK _ _ _ k) = k
+End
 
-Theorem raise_simps[simp]:
-  (raise e ctx).current_contract = ctx.current_contract ∧
-  (raise e ctx).call_stack = ctx.call_stack ∧
-  (raise e ctx).current_fc = ctx.current_fc with current_stmt := ExceptionK e
-Proof
-  rw[raise_def]
-QED
+val () = cv_auto_trans nextk_def;
 
-Theorem exception_raised_raise[simp]:
-  exception_raised (raise e ctx)
-Proof
-  rw[exception_raised_def]
-QED
+Definition stepk_def:
+  stepk (AK cx ak st k) =
+  case ak of
+     | Apply => apply cx st k
+     | ApplyExc ex => apply_exc cx ex st k
+     | ApplyTarget gv => apply_target cx gv st k
+     | ApplyTargets gvs => apply_targets cx gvs st k
+     | ApplyBaseTarget bv => apply_base_target cx bv st k
+     | ApplyTv tv => apply_tv cx tv st k
+     | ApplyVal v => apply_val cx v st k
+     | ApplyVals vs => apply_vals cx vs st k
+End
 
-Theorem pop_loop_simps[simp]:
-  (pop_loop ctx).current_contract = ctx.current_contract
-Proof
-  rw[pop_loop_def]
-  \\ CASE_TAC \\ rw[]
-QED
+val () = cv_auto_trans stepk_def;
 
-Theorem next_iteration_current_contract[simp]:
-  (next_iteration lp ctx).current_contract = ctx.current_contract
-Proof
-  rw[next_iteration_def]
-  \\ CASE_TAC \\ rw[]
-QED
+Definition cont_def:
+  cont ak = OWHILE (λak. nextk ak ≠ DoneK) stepk ak
+End
 
-(*
-Theorem expr_bound_acc:
-  (∀p e fns n fns'.
-     p = (e, fns) ∧
-     expr_bound (e,fns) = (n,fns') ⇒
-     fns ⊆ fns' ∧
-     (fns DIFF fns') ⊆ SND(expr_bound(e,∅)) ∧
-     ∀fns0. ∃fns1.
-       expr_bound (e,fns0) = (n,fns1) ∧
-       fns0 ⊆ fns1 ∧
-       (fns1 DIFF fns0) ⊆ SND(expr_bound(e,∅))) ∧
-  (∀p es fns n fns'.
-     p = (es, fns) ∧
-     expr_bound_list (es,fns) = (n,fns') ⇒
-     fns ⊆ fns' ∧
-     (fns DIFF fns') ⊆ SND(expr_bound(e,∅)) ∧
-     ∀fns0. ∃fns1.
-       expr_bound_list (es,fns0) = (n,fns1) ∧
-       fns0 ⊆ fns1 ∧
-       (fns1 DIFF fns0) ⊆ SND(expr_bound_list(es,∅)))
+Theorem eval_cps_eq:
+  (∀cx s st k.
+     cont (eval_stmt_cps cx s st k) =
+     cont ((
+       case eval_stmt cx s st
+         of (INL (), st1) => (AK cx Apply st1)
+          | (INR ex, st1) => (AK cx (ApplyExc ex) st1)
+     ) k)) ∧
+  (∀cx ss st k.
+     cont (eval_stmts_cps cx ss st k) =
+     cont ((
+       case eval_stmts cx ss st
+         of (INL (), st1) => (AK cx Apply st1)
+          | (INR ex, st1) => (AK cx (ApplyExc ex) st1)
+     ) k)) ∧
+  (∀cx g st k.
+     cont (eval_target_cps cx g st k) =
+     cont ((
+       case eval_target cx g st
+         of (INL gv, st1) => (AK cx (ApplyTarget gv) st1)
+          | (INR ex, st1) => (AK cx (ApplyExc ex) st1)
+     ) k)) ∧
+  (∀cx gs st k.
+     cont (eval_targets_cps cx gs st k) =
+     cont ((
+       case eval_targets cx gs st
+         of (INL gvs, st1) => (AK cx (ApplyTargets gvs) st1)
+          | (INR ex, st1) => (AK cx (ApplyExc ex) st1)
+     ) k)) ∧
+  (∀cx bt st k.
+     cont (eval_base_target_cps cx bt st k) =
+     cont ((
+       case eval_base_target cx bt st
+         of (INL bv, st1) => (AK cx (ApplyBaseTarget bv) st1)
+          | (INR ex, st1) => (AK cx (ApplyExc ex) st1)
+     ) k)) ∧
+  (∀cx nm body vs st k.
+     cont (eval_for_cps cx nm body vs st k) =
+     cont ((
+       case eval_for cx nm body vs st
+         of (INL (), st1) => (AK cx Apply st1)
+          | (INR ex, st1) => (AK cx (ApplyExc ex) st1)
+     ) k)) ∧
+  (∀cx e st k.
+     cont (eval_expr_cps cx e st k) =
+     cont ((
+       case eval_expr cx e st
+         of (INL tv, st1) => (AK cx (ApplyTv tv) st1)
+          | (INR ex, st1) => (AK cx (ApplyExc ex) st1)
+     ) k)) ∧
+  (∀cx es st k.
+     cont (eval_exprs_cps cx es st k) =
+     cont ((
+       case eval_exprs cx es st
+         of (INL vs, st1) => (AK cx (ApplyVals vs) st1)
+          | (INR ex, st1) => (AK cx (ApplyExc ex) st1)
+     ) k))
 Proof
-  ho_match_mp_tac expr_bound_ind
-  \\ rw[] \\ gvs[expr_bound_def]
-  \\ rpt (pairarg_tac \\ gvs[])
-  \\ gvs[SUBSET_DEF]
-
-  \\ TRY (
-    reverse CASE_TAC
+  ho_match_mp_tac evaluate_ind
+  \\ conj_tac >- rw[eval_stmt_cps_def, evaluate_def, return_def]
+  \\ conj_tac >- rw[eval_stmt_cps_def, evaluate_def, raise_def]
+  \\ conj_tac >- rw[eval_stmt_cps_def, evaluate_def, raise_def]
+  \\ conj_tac >- rw[eval_stmt_cps_def, evaluate_def, raise_def]
+  \\ conj_tac >- (
+    rw[eval_stmt_cps_def, evaluate_def, bind_def]
+    \\ CASE_TAC \\ reverse CASE_TAC
+    >- (
+      rw[cont_def]
+      \\ rw[Once OWHILE_THM, stepk_def, apply_exc_def] )
+    \\ rw[cont_def]
+    \\ rw[Once OWHILE_THM, stepk_def]
+    \\ rw[apply_tv_def, liftk1]
+    \\ CASE_TAC \\ reverse CASE_TAC
+    >- rw[Once OWHILE_THM, stepk_def, apply_exc_def]
+    \\ rw[raise_def]
+    \\ rw[Once OWHILE_THM, stepk_def, apply_val_def]
+    \\ rw[Once OWHILE_THM, stepk_def, SimpRHS] \\ gvs[]
+    \\ rw[apply_exc_def]
+    \\ rw[Once OWHILE_THM, stepk_def] )
+  \\ conj_tac >- rw[eval_stmt_cps_def, evaluate_def, raise_def]
+  \\ conj_tac >- (
+    rw[eval_stmt_cps_def, evaluate_def, bind_def]
+    \\ CASE_TAC \\ rw[cont_def] \\ reverse CASE_TAC
+    >- rw[Once OWHILE_THM, stepk_def, apply_exc_def]
+    \\ rw[Once OWHILE_THM, stepk_def, apply_tv_def, liftk1]
+    \\ reverse (Cases_on `x`) \\ simp[switch_BoolV_def, raise_def]
+    >- rw[Once OWHILE_THM, stepk_def, apply_exc_def]
+    \\ simp[return_def, Once OWHILE_THM, stepk_def]
+    \\ rw[apply_val_def, return_def, raise_def]
+    >- (
+      rw[Once OWHILE_THM, SimpRHS, stepk_def] \\ gvs[]
+      \\ rw[apply_def]
+      \\ rw[Once OWHILE_THM] )
+    >- (
+      rw[Once OWHILE_THM, SimpRHS, stepk_def] \\ gvs[]
+      \\ rw[apply_exc_def, Once OWHILE_THM] )
+    >- (
+      rw[Once OWHILE_THM, SimpRHS, stepk_def] \\ gvs[]
+      \\ Cases_on`v` \\ rw[apply_val_def, apply_exc_def]
+      \\ rw[Once OWHILE_THM] ))
+  \\ conj_tac >- (
+    rw[eval_stmt_cps_def, evaluate_def, bind_def]
+    \\ CASE_TAC \\ rw[cont_def] \\ reverse CASE_TAC
+    >- rw[Once OWHILE_THM, stepk_def, apply_exc_def]
+    >> rw[Once OWHILE_THM, stepk_def, apply_tv_def, liftk1]
+    \\ reverse CASE_TAC \\ reverse CASE_TAC
+    >- rw[Once OWHILE_THM, stepk_def, apply_exc_def]
+    >> rw[Once OWHILE_THM, stepk_def, liftk1, apply_val_def] )
+  \\ conj_tac >- (
+    rw[eval_stmt_cps_def, evaluate_def, bind_def]
+    \\ CASE_TAC \\ rw[cont_def] \\ reverse CASE_TAC
+    >- rw[Once OWHILE_THM, stepk_def, apply_exc_def]
+    >> rw[Once OWHILE_THM, stepk_def, apply_target_def]
+    \\ gvs[cont_def]
+    \\ first_x_assum drule \\ rw[]
+    \\ CASE_TAC \\ reverse CASE_TAC
+    >- rw[Once OWHILE_THM, stepk_def, apply_exc_def]
+    >> rw[Once OWHILE_THM, stepk_def, apply_tv_def, liftk1]
+    \\ CASE_TAC \\ reverse CASE_TAC
+    >- rw[Once OWHILE_THM, stepk_def, apply_exc_def]
+    >> rw[Once OWHILE_THM, stepk_def, apply_val_def, liftk1] )
+  \\ conj_tac >- (
+    rw[eval_stmt_cps_def, evaluate_def, bind_def, UNCURRY]
+    \\ CASE_TAC \\ gs[cont_def] \\ reverse CASE_TAC
+    >- rw[Once OWHILE_THM, stepk_def, apply_exc_def]
+    >> rw[Once OWHILE_THM, stepk_def, apply_base_target_def]
+    \\ qmatch_goalsub_rename_tac`AugAssignK1 p` \\ Cases_on`p`
+    \\ first_x_assum drule \\ rw[]
+    \\ CASE_TAC \\ reverse CASE_TAC
+    >- rw[Once OWHILE_THM, stepk_def, apply_exc_def]
+    >> rw[Once OWHILE_THM, stepk_def, apply_tv_def, liftk1]
+    \\ CASE_TAC \\ reverse CASE_TAC
+    >- rw[Once OWHILE_THM, stepk_def, apply_exc_def]
+    \\ gvs[oneline get_Value_def, toplevel_value_CASE_rator,
+           CaseEq"toplevel_value", CaseEq"prod", raise_def, return_def]
+    >> rw[Once OWHILE_THM, stepk_def, apply_val_def, liftk1])
+  \\ conj_tac >- (
+    rw[eval_stmt_cps_def, evaluate_def, bind_def, ignore_bind_def, UNCURRY]
+    \\ CASE_TAC \\ gs[cont_def] \\ reverse CASE_TAC
+    >- rw[Once OWHILE_THM, stepk_def, apply_exc_def]
+    >> rw[Once OWHILE_THM, stepk_def, apply_tv_def, liftk1]
+    \\ CASE_TAC \\ reverse CASE_TAC
+    >- rw[Once OWHILE_THM, stepk_def, apply_exc_def]
+    >> rw[Once OWHILE_THM, stepk_def, apply_def]
+    \\ first_x_assum drule \\ rw[]
+    \\ first_x_assum drule \\ rw[]
+    \\ gvs[switch_BoolV_def]
+    \\ IF_CASES_TAC \\ gvs[]
+    >- (
+      rw[apply_def, finally_def, bind_def, ignore_bind_def]
+      \\ gvs[push_scope_def, return_def]
+      \\ CASE_TAC \\ reverse CASE_TAC
+      >- (
+        rw[Once OWHILE_THM, stepk_def, apply_exc_def]
+        \\ CASE_TAC \\ CASE_TAC \\ rw[raise_def] )
+      \\ rw[Once OWHILE_THM, stepk_def, apply_def]
+      \\ CASE_TAC \\ CASE_TAC )
+    \\ IF_CASES_TAC \\ gvs[]
+    >- (
+      rw[apply_def, finally_def, bind_def, ignore_bind_def]
+      \\ gvs[push_scope_def, return_def]
+      \\ CASE_TAC \\ reverse CASE_TAC
+      >- (
+        rw[Once OWHILE_THM, stepk_def, apply_exc_def]
+        \\ CASE_TAC \\ CASE_TAC \\ rw[raise_def] )
+      \\ rw[Once OWHILE_THM, stepk_def, apply_def]
+      \\ CASE_TAC \\ CASE_TAC )
+    \\ qmatch_goalsub_abbrev_tac`Error str`
+    \\ gvs[push_scope_def, return_def]
+    \\ reverse $ Cases_on`x`
+    \\ rw[apply_def, finally_def, raise_def, ignore_bind_def, bind_def]
     \\ gvs[]
-    >- metis_tac[PAIR_EQ]
-    \\ first_assum(qspec_then`fns0`mp_tac)
-    \\ strip_tac \\ gvs[] \\ rw[]
-    \\ metis_tac[]
+    >- (
+      rw[pop_scope_def, return_def]
+      \\ rw[Once OWHILE_THM, stepk_def, apply_exc_def]
+      \\ rw[pop_scope_def, return_def] )
+    \\ Cases_on `v` \\ rw[apply_def]
+    \\ rw[Once OWHILE_THM, stepk_def, apply_exc_def]
+    \\ rw[pop_scope_def, return_def] )
+  \\ conj_tac >- (
+    rw[eval_stmt_cps_def, evaluate_def, ignore_bind_def, bind_def]
+    \\ CASE_TAC \\ gvs[cont_def] \\ reverse CASE_TAC
+    >- rw[Once OWHILE_THM, stepk_def, apply_exc_def]
+    >> rw[Once OWHILE_THM, stepk_def, apply_tv_def, liftk1]
+    \\ CASE_TAC \\ reverse CASE_TAC
+    >- rw[Once OWHILE_THM, stepk_def, apply_exc_def]
+    >> rw[Once OWHILE_THM, stepk_def, apply_val_def, bind_def, ignore_bind_def]
+    \\ CASE_TAC \\ reverse CASE_TAC
+    >- (
+      gvs[lift_option_def, option_CASE_rator, CaseEq"option",
+          return_def, raise_def]
+      \\ rw[Once OWHILE_THM, SimpRHS, stepk_def, apply_exc_def]
+      \\ gvs[]
+      \\ rw[Once OWHILE_THM, stepk_def, apply_exc_def] )
+    \\ CASE_TAC \\ reverse CASE_TAC
+    >- (
+      gvs[check_def, assert_def, raise_def]
+      \\ rw[Once OWHILE_THM, SimpRHS, stepk_def, apply_exc_def]
+      \\ gvs[]
+      \\ rw[Once OWHILE_THM, stepk_def, apply_exc_def] )
+    \\ rw[return_def]
+    \\ last_x_assum drule \\ rw[]
+    \\ last_x_assum drule \\ rw[]
+    \\ last_x_assum drule \\ rw[]
+    \\ gvs[]
+    \\ last_x_assum drule \\ rw[])
+  \\ conj_tac >- (
+    rw[eval_stmt_cps_def, evaluate_def, bind_def]
+    \\ CASE_TAC \\ gvs[cont_def] \\ reverse CASE_TAC
+    >- rw[Once OWHILE_THM, stepk_def, apply_exc_def]
+    \\ rw[Once OWHILE_THM, stepk_def, apply_tv_def, liftk1]
+    \\ rw[ignore_bind_def, bind_def, return_def]
+    \\ CASE_TAC \\ reverse CASE_TAC
+    >- rw[Once OWHILE_THM, stepk_def, apply_exc_def]
+    \\ rw[Once OWHILE_THM, stepk_def, apply_val_def]
+    \\ rw[Once OWHILE_THM, SimpRHS, stepk_def, apply_val_def]
+    \\ gvs[] \\ rw[apply_def]
+    \\ rw[Once OWHILE_THM, stepk_def] )
+  \\ conj_tac >- rw[eval_stmts_cps_def, evaluate_def, return_def]
+  \\ conj_tac >- (
+    rw[eval_stmts_cps_def, evaluate_def, return_def, ignore_bind_def, bind_def]
+    \\ CASE_TAC \\ gvs[cont_def] \\ reverse CASE_TAC
+    >- rw[Once OWHILE_THM, stepk_def, apply_exc_def]
+    \\ rw[Once OWHILE_THM, stepk_def, apply_def]
+    \\ gvs[]
+    \\ first_x_assum drule \\ rw[])
+  \\ conj_tac >- (
+    rw[eval_target_cps_def, evaluate_def, bind_def, return_def, UNCURRY]
+    \\ CASE_TAC \\ gvs[cont_def] \\ reverse CASE_TAC
+    >- rw[Once OWHILE_THM, stepk_def, apply_exc_def]
+    \\ rw[Once OWHILE_THM, stepk_def, apply_base_target_def] )
+  \\ conj_tac >- (
+    rw[eval_target_cps_def, evaluate_def, bind_def]
+    \\ CASE_TAC \\ gvs[cont_def] \\ reverse CASE_TAC
+    >- rw[Once OWHILE_THM, stepk_def, apply_exc_def]
+    \\ rw[Once OWHILE_THM, stepk_def, apply_targets_def, return_def] )
+  \\ conj_tac >- rw[eval_target_cps_def, evaluate_def, bind_def, return_def]
+  \\ conj_tac >- (
+    rw[eval_target_cps_def, evaluate_def, bind_def, return_def]
+    \\ CASE_TAC \\ gvs[cont_def] \\ reverse CASE_TAC
+    >- rw[Once OWHILE_THM, stepk_def, apply_exc_def]
+    \\ rw[Once OWHILE_THM, stepk_def, apply_target_def]
+    \\ first_x_assum drule \\ rw[]
+    \\ CASE_TAC \\ reverse CASE_TAC
+    >- rw[Once OWHILE_THM, stepk_def, apply_exc_def]
+    >> rw[Once OWHILE_THM, stepk_def, apply_targets_def] )
+  \\ conj_tac >- rw[eval_base_target_cps_def, evaluate_def, liftk1]
+  \\ conj_tac >- rw[eval_base_target_cps_def, evaluate_def, return_def]
+  \\ conj_tac >- (
+    rw[eval_base_target_cps_def, evaluate_def, bind_def, UNCURRY, return_def]
+    \\ CASE_TAC \\ gvs[cont_def] \\ reverse CASE_TAC
+    >- rw[Once OWHILE_THM, stepk_def, apply_exc_def]
+    \\ rw[Once OWHILE_THM, stepk_def, apply_base_target_def] )
+  \\ conj_tac >- (
+    rw[eval_base_target_cps_def, evaluate_def, bind_def, UNCURRY]
+    \\ CASE_TAC \\ gvs[cont_def] \\ reverse CASE_TAC
+    >- rw[Once OWHILE_THM, stepk_def, apply_exc_def]
+    \\ rw[Once OWHILE_THM, stepk_def, apply_base_target_def]
+    \\ qmatch_asmsub_rename_tac`INL p` \\ PairCases_on`p`
+    \\ first_x_assum drule \\ rw[]
+    \\ CASE_TAC \\ reverse CASE_TAC
+    >- rw[Once OWHILE_THM, stepk_def, apply_exc_def]
+    \\ rw[Once OWHILE_THM, stepk_def, apply_tv_def, liftk1]
+    \\ CASE_TAC \\ reverse CASE_TAC
+    >- rw[Once OWHILE_THM, stepk_def, apply_exc_def]
+    \\ qmatch_asmsub_rename_tac`get_Value tv`
+    \\ Cases_on`tv` \\ gvs[get_Value_def, raise_def, return_def]
+    \\ rw[Once OWHILE_THM, stepk_def, apply_val_def]
+    \\ CASE_TAC \\ reverse CASE_TAC
+    >- (
+      gvs[lift_option_def, option_CASE_rator, CaseEq"option",
+          raise_def, return_def]
+      \\ rw[Once OWHILE_THM, SimpRHS, stepk_def, apply_exc_def]
+      \\ gvs[]
+      \\ rw[Once OWHILE_THM, stepk_def, apply_exc_def] )
+    \\ rw[Once OWHILE_THM, SimpRHS, stepk_def, apply_exc_def]
+    \\ gvs[]
+    \\ rw[Once OWHILE_THM, stepk_def, apply_base_target_def] )
+  \\ conj_tac >- rw[eval_for_cps_def, evaluate_def, return_def]
+  \\ conj_tac >- (
+    rw[eval_for_cps_def, evaluate_def, ignore_bind_def, bind_def]
+    \\ CASE_TAC \\ gvs[cont_def] \\ reverse CASE_TAC \\ gvs[]
+    \\ first_assum drule \\ simp_tac std_ss [] \\ disch_then kall_tac
+    \\ rw[finally_def, try_def, bind_def]
+    \\ CASE_TAC \\ reverse CASE_TAC
+    >- (
+      rw[Once OWHILE_THM, stepk_def, apply_exc_def, finally_def]
+      \\ CASE_TAC \\ CASE_TAC
+      \\ rw[ignore_bind_def, bind_def, return_def, raise_def]
+      \\ CASE_TAC \\ CASE_TAC
+      \\ rw[return_def]
+      \\ last_x_assum drule \\ rw[]
+      \\ last_x_assum drule \\ rw[]
+      \\ gvs[finally_def, bind_def, try_def, CaseEq"prod", CaseEq"sum",
+             PULL_EXISTS, ignore_bind_def, return_def, raise_def]
+      \\ fsrw_tac[DNF_ss][]
+      \\ last_x_assum drule \\ rw[])
+    \\ rw[return_def]
+    \\ rw[Once OWHILE_THM, stepk_def, apply_def, ignore_bind_def, bind_def]
+    \\ CASE_TAC \\ reverse CASE_TAC
+    \\ rw[return_def]
+    \\ last_x_assum drule \\ rw[]
+    \\ gvs[finally_def, bind_def, try_def, CaseEq"prod", CaseEq"sum",
+           PULL_EXISTS, ignore_bind_def, return_def, raise_def]
+    \\ fsrw_tac[DNF_ss][]
+    \\ last_x_assum drule \\ rw[]
+    \\ last_x_assum drule \\ rw[])
+  \\ conj_tac >- rw[eval_expr_cps_def, evaluate_def, liftk1]
+  \\ conj_tac >- rw[eval_expr_cps_def, evaluate_def, liftk1]
+  \\ conj_tac >- (
+    rw[eval_expr_cps_def, evaluate_def, bind_def]
+    \\ CASE_TAC \\ gvs[cont_def] \\ reverse CASE_TAC
+    >- rw[Once OWHILE_THM, stepk_def, apply_exc_def]
+    \\ first_x_assum drule
+    \\ first_x_assum drule
+    \\ rw[]
+    \\ simp[switch_BoolV_def]
+    >> simp[Once OWHILE_THM, stepk_def, apply_tv_def, liftk1]
+    \\ IF_CASES_TAC \\ gvs[return_def]
+    >- rw[Once OWHILE_THM, stepk_def, apply_val_def]
+    \\ IF_CASES_TAC \\ gvs[return_def]
+    >- rw[Once OWHILE_THM, stepk_def, apply_val_def]
+    \\ simp[raise_def]
+    \\ Cases_on`x` \\ gvs[return_def]
+    >- (
+      Cases_on`v`
+      \\ rw[Once OWHILE_THM, stepk_def, apply_val_def, apply_exc_def]
+      \\ rw[Once OWHILE_THM, SimpRHS, stepk_def, apply_exc_def]
+      \\ gvs[]
+      \\ rw[Once OWHILE_THM, stepk_def, apply_val_def, apply_exc_def] )
+    \\ gvs[raise_def]
+    \\ rw[Once OWHILE_THM, stepk_def, apply_val_def, apply_exc_def] )
+  \\ conj_tac >- rw[eval_expr_cps_def, evaluate_def, return_def]
+  \\ conj_tac >- (
+    rw[eval_expr_cps_def, evaluate_def, ignore_bind_def, bind_def]
+    \\ CASE_TAC \\ gvs[cont_def] \\ reverse CASE_TAC
+    \\ gvs[]
+    \\ first_x_assum drule \\ rw[]
+    \\ CASE_TAC \\ reverse CASE_TAC
+    >- rw[Once OWHILE_THM, stepk_def, apply_exc_def]
+    \\ rw[return_def]
+    \\ rw[Once OWHILE_THM, stepk_def, apply_vals_def]
+    \\ rw[Once OWHILE_THM, SimpRHS, stepk_def]
+    \\ gvs[]
+    \\ simp[apply_tv_def]
+    \\ rw[Once OWHILE_THM, stepk_def] )
+  \\ conj_tac >- (
+    rw[eval_expr_cps_def, evaluate_def, bind_def]
+    \\ CASE_TAC \\ gvs[cont_def] \\ reverse CASE_TAC
+    >- rw[Once OWHILE_THM, stepk_def, apply_exc_def]
+    >> rw[Once OWHILE_THM, stepk_def, apply_tv_def]
+    \\ first_x_assum drule \\ rw[]
+    \\ CASE_TAC \\ reverse CASE_TAC
+    >- rw[Once OWHILE_THM, stepk_def, apply_exc_def]
+    >> rw[Once OWHILE_THM, stepk_def, apply_tv_def, liftk1]
+    \\ CASE_TAC \\ reverse CASE_TAC
+    >- rw[Once OWHILE_THM, stepk_def, apply_exc_def]
+    >> rw[Once OWHILE_THM, stepk_def, apply_val_def, liftk1]
+    \\ CASE_TAC \\ reverse CASE_TAC
+    \\ rw[return_def] )
+  \\ conj_tac >- (
+    rw[eval_expr_cps_def, evaluate_def, bind_def]
+    \\ CASE_TAC \\ gvs[cont_def] \\ reverse CASE_TAC
+    >- rw[Once OWHILE_THM, stepk_def, apply_exc_def]
+    >> rw[Once OWHILE_THM, stepk_def, apply_tv_def, liftk1]
+    \\ CASE_TAC \\ reverse CASE_TAC
+    >- rw[Once OWHILE_THM, stepk_def, apply_exc_def]
+    >> rw[Once OWHILE_THM, stepk_def, apply_val_def, liftk1]
+    \\ CASE_TAC \\ reverse CASE_TAC
+    \\ rw[return_def] )
+  \\ conj_tac >- (
+    rw[eval_expr_cps_def, evaluate_def, ignore_bind_def, bind_def]
+    \\ CASE_TAC \\ gvs[cont_def] \\ reverse CASE_TAC
+    \\ gvs[] \\ first_x_assum drule \\ rw[]
+    \\ CASE_TAC \\ reverse CASE_TAC
+    >- rw[Once OWHILE_THM, stepk_def, apply_exc_def]
+    >> rw[Once OWHILE_THM, stepk_def, apply_vals_def, bind_def, liftk1] )
+  \\ conj_tac >- (
+    rw[eval_expr_cps_def, evaluate_def, ignore_bind_def, bind_def]
+    \\ CASE_TAC \\ gvs[cont_def] \\ reverse CASE_TAC
+    \\ gvs[] \\ first_x_assum drule \\ rw[]
+    \\ CASE_TAC \\ reverse CASE_TAC
+    >- rw[Once OWHILE_THM, stepk_def, apply_exc_def]
+    >> rw[Once OWHILE_THM, stepk_def, apply_vals_def,
+          bind_def, ignore_bind_def, liftk1]
+    \\ qmatch_goalsub_abbrev_tac`check b c d`
+    \\ `check b c d = (INL (), d)`
+    by (
+      rw[check_def, assert_def, Abbr`b`]
+      \\ drule eval_exprs_length
+      \\ gvs[check_def, assert_def] )
+    \\ rw[] )
+  \\ conj_tac >- rw[eval_expr_cps_def, evaluate_def, raise_def]
+  \\ conj_tac >- (
+    rw[eval_expr_cps_def, evaluate_def, ignore_bind_def, bind_def,
+       no_recursion_def]
+    \\ CASE_TAC \\ gvs[cont_def] \\ reverse CASE_TAC
+    \\ reverse CASE_TAC
+    >- CASE_TAC
+    \\ reverse CASE_TAC
+    \\ reverse CASE_TAC
+    >- CASE_TAC
+    \\ CASE_TAC
+    \\ reverse CASE_TAC
+    >- CASE_TAC
+    \\ CASE_TAC
+    \\ rw[return_def]
+    \\ gvs[]
+    \\ first_assum (drule_then (drule_then (drule_then drule)))
+    \\ simp_tac std_ss [] \\ disch_then kall_tac
+    \\ CASE_TAC
+    \\ reverse CASE_TAC
+    >- rw[Once OWHILE_THM, stepk_def, apply_exc_def]
+    >> rw[Once OWHILE_THM, stepk_def, apply_vals_def, bind_def]
+    \\ CASE_TAC
+    \\ reverse CASE_TAC
+    \\ reverse CASE_TAC
+    >- (
+      CASE_TAC
+      \\ rw[Once OWHILE_THM, stepk_def, SimpRHS]
+      \\ gvs[apply_exc_def] \\ rw[Once OWHILE_THM] )
+    \\ reverse CASE_TAC
+    >- (
+      rw[Once OWHILE_THM, stepk_def, SimpRHS]
+      \\ gvs[apply_exc_def] \\ rw[Once OWHILE_THM] )
+    \\ reverse CASE_TAC
+    \\ reverse CASE_TAC
+    >- (
+      rw[Once OWHILE_THM, stepk_def, SimpRHS]
+      \\ gvs[apply_exc_def] \\ rw[Once OWHILE_THM] )
+    \\ rw[return_def, finally_def, try_def, bind_def]
+    \\ last_x_assum $ funpow 7 drule_then drule
+    \\ simp_tac std_ss [] \\ disch_then kall_tac
+    \\ reverse CASE_TAC
+    \\ reverse CASE_TAC
+    >- (
+      rw[Once OWHILE_THM, stepk_def, apply_exc_def, liftk1, finally_def]
+      \\ CASE_TAC \\ CASE_TAC \\ CASE_TAC \\ CASE_TAC
+      \\ gvs[ignore_bind_def, bind_def, pop_function_def, return_def,
+             set_scopes_def, lift_option_def, option_CASE_rator, CaseEq"option",
+             raise_def, push_function_def, o_DEF] )
+    \\ rw[Once OWHILE_THM, stepk_def, apply_def, liftk1]
+    \\ CASE_TAC
+    \\ reverse CASE_TAC
+    \\ gvs[push_function_def, return_def, o_DEF] )
+  \\ conj_tac >- rw[eval_expr_cps_def, evaluate_def, return_def]
+  \\ rw[eval_expr_cps_def, evaluate_def, bind_def]
+  \\ CASE_TAC \\ gvs[cont_def] \\ reverse CASE_TAC
+  >- rw[Once OWHILE_THM, stepk_def, apply_exc_def]
+  >> rw[Once OWHILE_THM, stepk_def, apply_tv_def, liftk1]
+  \\ CASE_TAC \\ reverse CASE_TAC
+  >- rw[Once OWHILE_THM, stepk_def, apply_exc_def]
+  >> rw[Once OWHILE_THM, stepk_def, apply_val_def]
+  \\ first_x_assum (drule_then drule) \\ rw[]
+  \\ CASE_TAC \\ reverse CASE_TAC
+  >- rw[Once OWHILE_THM, stepk_def, apply_exc_def]
+  \\ rw[return_def]
+  >> rw[Once OWHILE_THM, stepk_def, apply_vals_def]
+  >> rw[Once OWHILE_THM, SimpRHS, stepk_def, apply_vals_def]
+  \\ gvs[apply_vals_def]
+  \\ rw[Once OWHILE_THM, stepk_def]
+QED
 
-  \\ metis_tac[PAIR_EQ, SND, pair_CASES, NOT_IN_EMPTY]
+Definition fromk_def[simp]:
+  fromk (SOME (AK cx Apply st DoneK)) = (INL (), st) ∧
+  fromk (SOME (AK cx (ApplyExc ex) st DoneK)) = (INR ex, st) ∧
+  fromk _ = (INR $ Error "fromk", empty_state)
+End
 
+val () = cv_trans fromk_def;
 
-Theorem step_bound_stp_stmt_start:
-  ¬exception_raised ctx ∧
-  ctx.current_fc.current_stmt = StartK k ⇒
-  step_bound (step_stmt_start k ctx) < step_bound ctx
+Theorem cont_tr:
+  cont ak = if nextk ak = DoneK then SOME ak else cont (stepk ak)
 Proof
-  Cases_on`k` \\ rw[step_stmt_start_def]
-  \\ rw[step_bound_def]
-  \\ rpt(pairarg_tac \\ gvs[])
-  \\ TRY (gvs[fns_from_context_def] \\ NO_TAC)
-*)
+  simp[Once cont_def]
+  \\ simp[Once OWHILE_THM]
+  \\ IF_CASES_TAC \\ gs[]
+  \\ simp[Once cont_def]
+QED
 
-Definition step_stmt_till_exception_def:
-  step_stmt_till_exception ctx =
-  if exception_raised ctx then ctx
-  else step_stmt_till_exception (step_stmt ctx)
-Termination
-  cheat
-(*
-  WF_REL_TAC`measure step_bound`
-  \\ rw[step_stmt_def, Excl"APPEND"]
-  \\ CASE_TAC
+val cont_tr_pre_def = cv_trans_pre cont_tr;
+
+Theorem IS_SOME_cont:
+  IS_SOME (cont ak) ⇔
+  ∃n. nextk (FUNPOW stepk n ak) = DoneK
+Proof
+  rw[cont_def, OWHILE_def]
+QED
+
+Theorem cont_pre_IS_SOME_cont:
+  cont_pre ak ⇔ IS_SOME (cont ak)
+Proof
+  EQ_TAC
   >- (
-    CASE_TAC
-    >- ( rw[step_bound_def] \\ pairarg_tac \\ fs[])
-    >- ( rw[step_bound_def]
-      \\ pairarg_tac \\ gvs[]
-      \\ gs[continue_loop_def]
-      \\ Cases_on`ctx.current_fc.name` \\ gs[]
-      >- (
-        gs[fns_from_context_def]
-        \\ pairarg_tac \\ gvs[] )
-      \\ pairarg_tac \\ gvs[]
-      \\ pairarg_tac \\ gvs[]
-      \\ gs[pop_scope_def]
-      \\ Cases_on`ctx.current_fc.scopes` \\ gvs[]
-      >- gs[fns_from_context_def]
-      \\ IF_CASES_TAC
-      >- gs[exception_raised_def]
-      \\ cheat )
-    >- ( rw[step_bound_def]
-      \\ pairarg_tac \\ gs[]
-      \\ gs[break_loop_def]
-      \\ Cases_on`ctx.current_fc.name` \\ gs[]
-      >- (
-        gs[fns_from_context_def]
-        \\ pairarg_tac \\ gvs[] )
-      \\ pairarg_tac \\ gvs[]
+    qid_spec_tac`ak`
+    \\ ho_match_mp_tac (theorem "cont_pre_ind")
+    \\ rw[cont_def, OWHILE_def] \\ gs[]
+    >- (
+      first_x_assum(qspec_then`SUC n`mp_tac)
+      \\ rw[FUNPOW] )
+    \\ first_x_assum(qspec_then`0`mp_tac)
+    \\ rw[] )
+  \\ rw[IS_SOME_cont]
+  \\ pop_assum mp_tac
+  \\ qid_spec_tac`ak`
+  \\ Induct_on`n` \\ rw[]
+  >- rw[cont_tr_pre_def]
+  \\ rw[Once cont_tr_pre_def]
+  \\ first_x_assum irule
+  \\ gs[FUNPOW]
+QED
 
+Theorem eval_stmts_eq_cont_cps:
+  eval_stmts cx body st = fromk $ cont (eval_stmts_cps cx body st DoneK)
+Proof
+  Cases_on`eval_stmts cx body st`
+  \\ qmatch_goalsub_rename_tac`res,st1`
+  \\ qspecl_then[`cx`,`body`,`st`,`DoneK`]mp_tac(cj 2 eval_cps_eq)
+  \\ simp[cont_def] \\ strip_tac
+  \\ simp[Once OWHILE_THM]
+  \\ IF_CASES_TAC
+  >- (Cases_on `res` \\ gvs[])
+  \\ CASE_TAC \\ simp[]
+QED
 
-    \\ cheat )
-    >- ( rw[step_bound_def] \\ rpt(pairarg_tac \\ gvs[]))
-    >- ( rw[step_bound_def] \\ rpt(pairarg_tac \\ gvs[]))
-    >- ( rw[step_bound_def] \\ rpt(pairarg_tac \\ gvs[]))
-    >- ( rw[step_bound_def] \\ rpt(pairarg_tac \\ gvs[]))
-    >- ( rw[step_bound_def] \\ rpt(pairarg_tac \\ gvs[raise_def]))
-    *)
-End
+val call_external_function_pre_def = call_external_function_def
+     |> SRULE [eval_stmts_eq_cont_cps]
+     |> cv_auto_trans_pre;
 
-val () = cv_auto_trans step_stmt_till_exception_def;
+Theorem call_external_function_pre[cv_pre]:
+  call_external_function_pre am cx args vals body
+Proof
+  rw[call_external_function_pre_def]
+  \\ rw[cont_pre_IS_SOME_cont]
+  \\ qmatch_goalsub_abbrev_tac`eval_stmts_cps cx ss st k`
+  \\ qspecl_then[`cx`,`ss`,`st`,`k`]mp_tac  $ cj 2 eval_cps_eq
+  \\ rw[]
+  \\ CASE_TAC
+  \\ CASE_TAC
+  \\ rw[Abbr`k`, cont_def]
+  \\ rw[Once OWHILE_THM]
+QED
 
-Definition process_exception_def:
-  process_exception (ExceptionK (ExternalReturn v)) = INL v ∧
-  process_exception (ExceptionK (AssertException msg)) =
-    INR ("Assertion Failed: " ++ msg) ∧
-  process_exception (ExceptionK (RaiseException msg)) =
-    INR ("Exception Raised: " ++ msg) ∧
-  process_exception (ExceptionK (Error msg)) = INR msg ∧
-  process_exception _ = INR "process_exception"
-End
-
-val () = cv_auto_trans process_exception_def;
-
-Definition step_external_function_def:
-  step_external_function tx ctr bal params body =
-   (case bind_arguments params tx.args of
-      SOME env =>
-      (let fc = initial_function_context tx.function_name env body in
-       let ctx = initial_execution_context tx ctr bal fc in
-       let ctx = step_stmt_till_exception ctx in
-       let ctr = ctx.current_contract in
-         (process_exception ctx.current_fc.current_stmt, ctr))
-    | _ => (INR "external bind_arguments", ctr))
-End
-
-val () = cv_auto_trans step_external_function_def;
-
-Definition external_call_contract_def:
- external_call_contract ctr bal tx =
- case lookup_function tx.function_name External ctr.src of
-   NONE => (INR "lookup_function External", ctr)
-  (* TODO: update balances on return *)
- | SOME (params, _, body) => step_external_function tx ctr bal params body
-End
-
-val () = cv_auto_trans external_call_contract_def;
-
-Definition external_call_def:
-  external_call ms tx =
-  let addr = tx.target in
-  case ALOOKUP ms.contracts addr of NONE => (INR "no contract at addr", ms)
-     | SOME ctr =>
-  (* TODO: update balances on return *)
-  case external_call_contract ctr ms.balances tx of
-       (res, ctr) =>
-       (res, ms with contracts updated_by CONS (addr, ctr))
-End
-
-val () = cv_auto_trans external_call_def;
-
-Definition load_contract_def:
-  load_contract ms tx ts =
-  let addr = tx.target in
-  let ctr = <|src := ts; globals := initial_globals (type_env ts) ts |> in
-  case lookup_function tx.function_name Deploy ts of
-    | NONE => INR "no constructor"
-    | SOME (params, _, body) => (
-    (* TODO: update balances on return *)
-      case step_external_function tx ctr ms.balances params body of
-      | (INR msg, _) => INR msg
-      | (INL _, ctr) => INL $ ms with contracts updated_by (CONS (addr, ctr))
-    )
-End
+val () = cv_auto_trans call_external_def;
 
 val () = cv_auto_trans load_contract_def;
 
